reorganize: only definitions in densem.v. working through examples with if

VerseRocq/verse/densem/densem.v
@@ -1,7 +1,5 @@
 Require Import Imports.
 
-
-
 From Stdlib Require Lists.List.
 From Stdlib Require Import Classes.EquivDec.
 Import ssreflect.
@@ -15,12 +13,11 @@ Require syntax.mini.
 Require Import PFun.
 Require Import structures.Sets.
 Import structures.List.
-Import structures.Monad.
-Require Import structures.Laws.
 
-Require Import densem.Dom.
-Require Import densem.tenv.  (* environments are total *)
-Require Import densem.envSet. (* ENV , hide, constraints *)
+Require Export densem.Dom.
+Require Export densem.tenv.  (* environments are total *)
+Require Export densem.envSet. (* def of ENV , hide, constraints *)
+Require Export densem.squash.
 
 Import mini.MiniNotation.
 Import SetNotations.
@@ -28,27 +25,16 @@ Import SetMonadNotation.
 Import List.ListNotations.
 Import ListMonadNotation.
 Import EnvNotation.
-Import ENVNotation.
+Import envSetNotation.
 
-
-Open Scope monad_scope.
 Open Scope list_scope.
 Open Scope mini_expr_scope.
 Open Scope env_scope.
 Open Scope set_scope.
 
-Notation "r ≈ x ≈ ⟨ k ⟩" := ((r ≈ ⟪ x ⟫) ∩ (x ≈ ⟨ k ⟩)).
 
 (* ---------------------------------------------- *)
 
-(* This axiom is BAD. But convenient for now.... *)
-Axiom empty_dec : forall {A} (s : P A), 
-    { s ≃ ∅ } + { ~ (s ≃ ∅) }.
-
-Definition is_Empty_set {A} (s : P A) : bool := 
-  match empty_dec s with 
-  | left _ => true | right _ => false 
-  end.
 
 
 Ltac set_crunch :=
@@ -69,6 +55,10 @@ Ltac set_crunch :=
         inv H; crunch
     | [ H : ?ρ ∈ (when ?x ?k) |- _ ] =>
         inv H; crunch
+    | [ H : ?ρ ∈ ∅ |- _] => 
+        inv H
+    | [ H : ?ρ ∈ (fun x => _ ) |- _ ] =>
+        inv H; crunch
     | [ H : ?ρ ∈ (?x ≈ ?k) |- _ ] =>
         inv H; crunch
     | [ H : ?ρ ∈ (?x ≉ ?k) |- _ ] =>
@@ -81,47 +71,12 @@ Ltac set_crunch :=
 
 (* --------------------------------------------------- *)
 
-Definition VAL := P value.
+Notation VAL := (P value).
 
 Import mini.MiniNotation.
-
+Notation "⟅ r ⟆" := (Scope.singleton r).
 (* distinguished result variable (0) *)
 Definition r : Ident := mini.Test.r.
-Definition rs : Scope.t := Scope.singleton r.
-Notation "⟅ r ⟆" := (Scope.singleton r).
-(* another variable (1) *)
-Definition x := mini.Test.x.
-Definition y := mini.Test.y.
-
-
-(* This is a bit of a hack. For examples, we special case the variables
-   x,y, and y when simplifying environment lookups *)
-
-Ltac rewrite_env := 
-  repeat match goal with 
-    | [ |- context[ (?x |-> ?v , ?rho) ?x ] ] => 
-        rewrite extend_lookup_same
-    | [ |- context[ (x |-> ?v , ?rho) r ] ] => 
-        rewrite extend_lookup_diff;
-        [rewrite PeanoNat.Nat.eqb_neq;easy|]
-    | [ |- context[ (y |-> ?v , ?rho) r ] ] => 
-        rewrite extend_lookup_diff;
-        [rewrite PeanoNat.Nat.eqb_neq;easy|]
-    | [ |- context[ (r |-> ?v , ?rho) x ] ] => 
-        rewrite extend_lookup_diff;
-        [rewrite PeanoNat.Nat.eqb_neq;easy|]
-    | [ |- context[ (r |-> ?v , ?rho) y ] ] => 
-        rewrite extend_lookup_diff;
-        [rewrite PeanoNat.Nat.eqb_neq;easy|]
-    | [ |- context[ (y |-> ?v , ?rho) x ] ] => 
-        rewrite extend_lookup_diff;
-        [rewrite PeanoNat.Nat.eqb_neq;easy|]
-    | [ |- context[ (x |-> ?v , ?rho) y ] ] => 
-        rewrite extend_lookup_diff;
-        [rewrite PeanoNat.Nat.eqb_neq;easy|]
-  end.
-
-
 
 (* -------------- atomic expressions  ---------------- *)
 
@@ -166,20 +121,23 @@ Definition MINUS {A} (d1 : list (P A)) (d2: list (P A)) :
   ρ2 <- d2 ;;
   [ρ1 - ρ2].
  
-Definition IF2 {A B} : list (P A) -> list (P B) -> list (P B) := liftM2 If2.
+Definition IF2 {A B} (d1 : list (P A)) (d2: list (P B)) : list (P B) := 
+  ρ1 <- d1 ;;
+  ρ2 <- d2 ;;
+  [If2 ρ1 ρ2].
 
 Infix "*" := UNIFY.
 
-(* --------- pick/sequence ----------- *)
+Definition UNIONLIST {A} : list (P A) -> (P A) := 
+  List.fold_right Union ∅.
 
-Definition Cons {A} := (fun (V : P A) (VS : P (list A)) => 
-    v  ⭅ V  ;;  vs ⭅ VS ;; ⌈ v :: vs⌉).
+
+(* --------- pick/sequence ----------- *)
 
 (* This operation is liftM2 snoc *)
 Definition Snoc {A} := (fun (VS : P (list A)) (V : P A) => 
     vs ⭅ VS ;;  v  ⭅ V  ;; ⌈ vs ++ [v]⌉).
    
-
 (* The set of all first elements from a list. *)
 (*   {{ v | (v :: _) <- V }}   *)
 Definition Head {A} (V : P (list A)) : P A := 
@@ -188,7 +146,6 @@ Definition Head {A} (V : P (list A)) : P A :=
   | v :: _ => ⌈ v ⌉
   | _ => ∅
   end. 
-
 
 Fixpoint pick {A} (xs : list (P A)) : P (list A) := 
   match xs with 
@@ -202,34 +159,6 @@ Fixpoint pickl {A} (xs : list (list A)) : list (list A) :=
   match xs with 
   | nil => [ [] ]
   | V :: VS =>  v <- V ;; vs <- pickl VS ;; [ v :: vs ] 
-  end.
-
-(* ------------- squash -------------- *)
-
-(* squash using axiom *)
-Definition squash {A} (xs : list(P A)) : list (P A) := 
-  x <- xs ;; if is_Empty_set x then [x] else [].
-
-(* left to right squash, doesn't require axiom, but cannot 
-   produce a list.
-   fold_left allows us to use snoc in the definition of ALL
-*)
-Definition squash_fold_left {A B} (f : P A -> P B -> P A) : 
-  list (P B) -> P A -> P A := 
-  List.fold_left (fun bs x => If3 x (f bs x) bs).
-
-(* Find the first nonempty set, or an empty set if none exist. *)
-Definition first {A} (VS : list (P A)) : P A := 
-  squash_fold_left (fun xs x => x) VS ∅.
-
-(* squashing and picking at the same time *)
-(* doesn't require axiom *)
-Fixpoint squash_pick {A} (xs : list (P A)) : P (list A) := 
-  match xs with 
-  | nil => ⌈ [] ⌉
-  | V :: VS => If3 V  
-               (Cons V (squash_pick VS))
-               (squash_pick VS)
   end.
 
 (* --------- dodgy union ----------- *)
@@ -248,7 +177,7 @@ Definition Pointwise_Unions {A} : list (list (P A)) -> list (P A) :=
 (* another version of the dodgy big union *)
 Definition DODGY_UNIONS {A} (VVS : P (list (P A))) : list (P A) := 
   i <- allNums ;;
-  let VS : P (P A) := fmap (fun VS => List.nth i VS ∅) VVS in
+  let VS : P (P A) := Sets.map (fun VS => List.nth i VS ∅) VVS in
   [ ⨃ VS ].
 
 Infix "⩅" := pointwise_union (at level 70).
@@ -285,7 +214,7 @@ Definition apply (f : value) (v : value) : list VAL :=
 *)
 Definition APPi (e1 : mini.Expr) (e2 : mini.Expr) (i : nat) : ENV := 
   fun ρ => 
-    List.nth_error (apply (evalA e1 ρ) (evalA e2 ρ)) i = Some (ret (ρ r)).
+    List.nth_error (apply (evalA e1 ρ) (evalA e2 ρ)) i = Some (⌈ ρ r ⌉).
 
 Definition APPi' (e1 : mini.Expr) (e2 : mini.Expr) (i : nat) : ENV := 
   fun ρ => 
@@ -297,7 +226,7 @@ Definition APPi' (e1 : mini.Expr) (e2 : mini.Expr) (i : nat) : ENV :=
    We need to iterate only over each partial function *)
 Definition APP (e1 : mini.Expr) (e2 : mini.Expr) : list ENV := 
   i <- allNums ;;
-  ret (APPi e1 e2 i).
+  [APPi e1 e2 i].
 
 (* --- semantics of ALL / ONE for dest passing --------- *)
 
@@ -306,7 +235,7 @@ Definition APP (e1 : mini.Expr) (e2 : mini.Expr) : list ENV :=
 (* {{  (v, Δ') | ρ ∈ Δ , v = ρ.r, Δ' = (Δ ∩ {{ r = v }}) \ r  }} *)
 Definition extract r (Δ : ENV) : P (value * ENV) := 
   ρ ⭅ Δ ;;
-  ret ( ρ r , (Δ ∩ r ≈ ⟨ρ r⟩) \ ⟅r⟆ ).
+  ⌈ (ρ r , (Δ ∩ r ≈ ⟨ρ r⟩) \ ⟅r⟆) ⌉.
 
 (* The set of results in Δ that could be produced by environments 
    consistent with ρ *)
@@ -372,16 +301,57 @@ Fixpoint combine (xs : list ENV) : P (list value * ENV) :=
   [E{a}[1] \{xs} E{a}[0]                        ]             + … +
   [E{a}[n] \{xs} E{a}[0] \{xs} … \{xs} E{a}[n-1]])
 *)
-Fixpoint try (xs : Scope.t) (Δs : list ENV) : list ENV * ENV := 
-  let step := fun '(envs, avoid) Δi => 
-                (envs ++ [Δi - avoid], avoid ∪ (Δi \ xs)) in
-  List.fold_left step Δs ([],∅).
 
-Definition IF_TIM xs S1 S2 S3 := 
-    let (success, avoid) := try xs S1 in 
-     (SEQ success (S2 [\] xs)) ++
-     (SEQ [Total_set - avoid] S3).
 
+(* Tims version in Euv semantics 
+
+Euv{if(a){b}else{c}} := 
+   [A[0], 
+    A[1]\A[0], ..., 
+    A[n]\A[0]\A[1]\...\ A[n-1]] * B + 
+   [P(Env)\A[0]\A[1]\...\A[n]] * C
+where A:=Epq{a}-a -{p,q}
+where B:=Euv{b}-a-b-{p,q}
+where C:=Euv{c}-a-c-{p,q}
+where p&q fresh, n:=Length(Epq{a})
+
+Questions:
+1. should it be
+   where C:=Euv{c}-c
+   i.e. variables bound in a don't scope over c
+        p,q are fresh for c, and not input to Euv
+2. Aren't we subtracting a variables from A and B too early?
+   They need to communicate. We should only subtract
+   after the * has been calculated.
+2'. But, the a variables aren't bound in C, so we can 
+   subtract them before we do the unification
+3. Let's replace A[i]\A[0]...\A[i-i] with 
+     A[i]\(A[0] ∪ ... ∪ A[i-1])
+
+Proposed update:
+
+Euv{if(a){b}else{c}} := 
+   ([A[0], 
+     A[1]\A[0], 
+     ..., 
+     A[n]\(A[0] ∪ A[1] ... ∪ A[n-1])] * B)-a + 
+   [P(Env)\(A[0] ∪ A[1] ... ∪ A[n])-a] * C
+where A:=Epq{a}-{p,q}
+where B:=Euv{b}-b
+where C:=Euv{c}-c
+where p&q fresh, n:=Length(Epq{a})
+
+*)
+
+Fixpoint try (a : Scope.t) (A : list ENV) : list ENV * ENV := 
+  let step := fun '(envs, avoid) Ai => 
+                (envs ++ [Ai - avoid], avoid ∪ Ai) in
+  List.fold_left step A ([],∅).
+
+Definition IF_TIM a (A B C : list ENV) : list ENV := 
+    let (success, avoid) := try a (A [\] ⟅r⟆) in 
+     ((success * B) [\] a) ++
+     ([(Total_set - avoid) \ a] * C).
 
 (* Koen's encoding of if *)
 
@@ -393,33 +363,26 @@ if e1 e2 e3 =
 *)
 
 (* Translated to DPS style, with distinguished result r *)
-Definition koen_if e1 e2 e3 : mini.Expr := 
+Definition koen_if y e1 e2 e3 : mini.Expr := 
   mini.DefineV y :>:
   y :=: mini.One ( (e1 :>: (r :=: mini.Array [])) :|: r :=: 0 ) :>:
   (y :=: mini.Array [] :>: e2) :|: (y :=: 0 :>: e3).
 
-Definition IF_KOEN (xs:Scope.t) (S1 S2 S3 : list ENV) : list ENV :=
-  SEQ [ONE( SEQ S1 [r ≈ ⟨mkTup []⟩] ++ [r≈⟨Int 0⟩])]
+Definition IF_KOEN y (xs:Scope.t) (S1 S2 S3 : list ENV) : list ENV :=
+  let D1 := ONE( SEQ S1 [r ≈ ⟨mkTup []⟩] ++ [ r ≈ ⟨Int 0⟩]) in
+  SEQ [ (y ≈ fun ρ => ρ r) ∩ D1 ]
       (SEQ [y≈⟨mkTup[]⟩] S2) ++ (SEQ [y ≈⟨Int 0⟩] S3).
 
 (* Simon's version of If *)
 
-Definition UNIONLIST : list ENV -> ENV := 
-  List.fold_right Union ∅.
-
 Definition IF_SPJ (xs:Scope.t) (S1 S2 S3 : list ENV) : list ENV :=
     let GOOD := UNIONLIST (S1 [\] ⟅ r ⟆) in
-    (List.map (fun D => D ∩ GOOD) S2) ++ 
+    ((List.map (fun D => D ∩ GOOD) S2) [\] xs) ++ 
     (List.map (fun D => D - GOOD) S3).
-
-(* E [if (x=1|x=2) { x } { 0 }] = [ {r=1,x=1} | {r=2,x=2} | {r=0,x<>1,2} *)
-
-
-Definition if_iter := mini.If3 (x :=: 1 :|: x :=: 2) x 0.
 
 (* ----------- non-dodgy dest passing style -------------- *)
 
-Module D_LS. 
+Module DLS. 
 
 Fixpoint E (e : mini.Expr) : list ENV := 
 
@@ -440,7 +403,7 @@ Fixpoint E (e : mini.Expr) : list ENV :=
 
   | mini.Fail => []  
 
-  | mini.Choice e1 e2 => E e1 ++ E e2
+  | mini.Choice e1 e2 => B e1 ++ B e2
 
   | mini.Unify e1 e2 => 
       E e1 * E e2
@@ -455,10 +418,11 @@ Fixpoint E (e : mini.Expr) : list ENV :=
     let xs := mini.I a in 
     let (success, avoid) := try xs (E a) in 
 
-     (SEQ success (E b [\] xs)) ++
-     (SEQ [Total_set - avoid] (E c))
+     ((SEQ success (B b)) [\] xs) ++
+     (SEQ [Total_set - avoid] (B c))
 
 
+  (* TODO: should this be E or B *)
   | mini.All a => 
       [ ALL (E a) \ mini.I a ] 
 
@@ -470,66 +434,25 @@ Fixpoint E (e : mini.Expr) : list ENV :=
   | _ => [ ] 
   end.
 
-End D_LS.
-
-Module D_LS_Theory.
-
-Import D_LS.
+Definition  B (e : mini.Expr) :list ENV := 
+    Δ <- E e ;; [Δ \ mini.I e]. 
 
 Lemma E_Var (i:Ident) : E i = [ fun ρ => ρ r = ρ i ]. reflexivity. Qed.
 Lemma E_One e : E (mini.One e) = [ ONE (E e) \ mini.I e ]. reflexivity. Qed.
-Lemma E_Choice e1 e2 : E (e1 :|: e2) = (E e1) ++ (E e2). reflexivity. Qed.
+Lemma E_Choice e1 e2 : E (e1 :|: e2) = (B e1) ++ (B e2). reflexivity. Qed.
 Lemma E_Seq e1 e2 : E (e1 :>: e2) = (E e1 [\] ⟅r⟆) * E e2. reflexivity. Qed.
 Lemma E_Unify e1 e2 : E (e1 :=: e2) = E e1 * E e2. reflexivity. Qed.
 
 Create HintDb E.
 Hint Rewrite E_Var E_One E_Choice E_Seq E_Unify : E.
 
-(* if(a){b}else{c} <=> if(a){b}else{:false} | if(a){:false}else{c} *)
-Lemma opinionated_if a b c: 
-  E(mini.If3 a b c) =  E( mini.If3 a b mini.Fail :|: mini.If3 a mini.Fail c).
-Proof. 
-  unfold E. fold E.
-  destruct (try (mini.I a) (E a)) as [success avoid].
-  replace (SEQ [Total_set - avoid] []) with ([] : list ENV).
-  2 : { cbn. auto. } 
-  rewrite -> List.app_nil_r.
-  replace (SEQ success ([] [\] mini.I a)) with ([] : list ENV).
-  2: { cbn. unfold SEQ, UNIFY. cbn.
-       admit. } 
-  rewrite -> List.app_nil_l. auto.
-Admitted.
-
-
-(* 
-
-if e1 e2 e3 =
-  exists y; 
-  y = one{ (e1; z=⟨⟩) | z=0 }@z;
-  (y=⟨⟩; e2) | (y=0; e3)
-
-koen_if =
-  fun e1 e2 e3 : mini.Expr =>
-  ∃ y :>: 
-  y :=: mini.One (e1 :>: r :=: mini.Array [] :|: r :=: 0) :>: 
-  y :=: mini.Array [] :>: e2 :|: y :=: 0 :>: e3
-*)
-
-(*
-= [ D ⋂ GOOD | D ∈ Ed[e2] ] ++
-  [ D \ GOOD | D ∈ Ed[e3] ]
-where
-  GOOD :: ENV = UNIONLIST (map hide(r) Ed[e1])
-
-*)
-
-End D_LS_Theory.
+End DLS.
 
 
 (* ------------------------------------------------------ *)
 (* ------  Fig 17 D-LS (using dodgy union) -------------- *)
 
-Module DLS_OLD.
+Module DLS_Dodgy.
 
 
 Fixpoint E (e : mini.Expr) : list ENV := 
@@ -556,13 +479,8 @@ Fixpoint E (e : mini.Expr) : list ENV :=
 
   | mini.ApplyD e1 e2 => APP e1 e2
 
-  | mini.If3 e1 e2 e3 =>  
-
-    let Y  := mini.I e1 in 
-    let Δ1 := first (E e1) \ Scope.singleton r in
-
-     (Δ2 <- E e2 ;; [(Δ1 ∪ Δ2) \ Y])  ⩅
-     (Δ3 <- E e3 ;; [Δ3 - Δ1 \ Y])
+  | mini.If3 e1 e2 e3 => 
+      IF_SPJ (mini.I e1) (E e1) (E e2) (E e3)
 
   | mini.All a => 
        [ ALL (B a)  ] 
@@ -576,668 +494,19 @@ Fixpoint E (e : mini.Expr) : list ENV :=
   end.
 
 
-End DLS_OLD.
+End DLS_Dodgy.
 
-
-
-
-(* ---- examples / theory about extract / squash_pick ----- *)
-
-Lemma squash_pick_singleton {A} (v : A) : 
-  squash_pick [ ⌈ v ⌉ ] = ⌈ [v] ⌉.  
-  cbn.
-  set_simpl.
-  unfold Cons. set_simpl.
-  done.
-Qed.
-
-Example squash_pickExample :
-  squash_pick [  ⌈ (Int 0) ⌉ ; ⌈ (Int 1) ⌉ ] = 
-    (⌈ [ Int 0 ; Int 1 ] ⌉).
-cbn. set_simpl.
-unfold Cons. set_simpl.
-done.
-Qed.
-
-Lemma squash_pick_two_example :
-  squash_pick [ ⌈ (Int 0) ⌉ ∪ ⌈ (Int 1) ⌉ ] = 
-               (⌈ [ Int 0 ] ⌉ ∪ ⌈ [ Int 1 ] ⌉).
-Proof.
-  cbn. set_simpl.
-  unfold squash_fold_left.
-  unfold List.fold_left.
-Admitted.
-
-
-Lemma extract_one {v} : 
-  extract r (r ≈ ⟨ v ⟩) = ⌈ (v, Total_set) ⌉.
-Proof. 
-eapply set_extensionality. intro ρ.
-unfold extract. 
-set_simpl.
-split.
-- move=>h.
-  set_crunch.
-  set_simpl.
-  f_equal.
-- destruct ρ as [w Δ].
-  intro h. inv h.
-  exists (r |-> v).
-  set_simpl.
-  done.
-Qed. 
-
-Lemma extract_example {k} :
-  extract r (x ≈ ⟨ k ⟩ ∩ r ≈ ⟨ k ⟩) = 
-    ⌈ (k, x ≈ ⟨ k ⟩) ⌉.
-Proof.
-  unfold extract.
-  eapply set_extensionality. intros [v Δ].
-  set_simpl.
-  split.
-  + intros h.
-    inv h.
-    set_crunch.
-    inv H.
-    repeat rewrite H2.  clear H2.
-    f_equal.
-    set_simpl.
-    rewrite constrain_eq_hide_two. done. done.
-  + intro h. inv h.
-    exists (x |-> k, r |-> k).
-    set_simpl.
-    rewrite_env.
-    rewrite constrain_eq_hide_two. done. done.
-Qed. 
-
-Lemma extract_two :
-  extract r (r ≈ ⟨ Int 0 ⟩ ∪ (r ≈ ⟨ Int 1 ⟩)) = 
-    (ret (Int 0, Total_set) ∪ ret (Int 1, Total_set)).
-Admitted.
-
-
-Lemma bcp_example : 
-  ALL [x ≈ ⟨ Int 0 ⟩ ∩ r ≈ ⟨ Int 0 ⟩] = 
-      ((x ≈ ⟨ Int 0 ⟩ ∩ r ≈ ⟨mkTup [Int 0]⟩) ∪
-       (x ≉ ⟨ Int 0 ⟩ ∩ r ≈ ⟨mkTup []⟩)).
-Proof.
-  unfold ALL.
-  apply set_extensionality. intros ρ.
-  unfoldIn.
-  unfold consistent_results.
-  list_simpl.
-  rewrite extract_example.
-  set_simpl.
-  unfold squash_pick.
-  remember (when (ρ ∈ x ≈ ⟨ Int 0 ⟩) ⌈ Int 0 ⌉) as ϕ.
-  split.
-  + intro h. 
-    crunch.
-    unfold If3 in H.
-    inv H. 
-    ++ Sets.set_crunch.
-       unfold Cons in H1.
-       Sets.set_crunch.
-       inv H2.
-       rewrite H3.
-       left. split; eauto.
-    ++ unfold when, guard in H1.
-       Sets.set_crunch.       
-       inv H.
-       have F: ⟨ ρ ∈ x ≈ ⟨ Int 0 ⟩ ⟩ = ∅. admit.
-       right. split; auto.
-       intro h.
-       admit.       
-  + intro h. inv h.
-    ++ set_crunch. 
-       exists [Int 0].
-       split; auto.
-       cbn. unfold constrain_eq. 
-Admitted.
-(*
-rewrite H1.
-       left.
-       have hh: (Int 0 = Int 0) = True. { apply propositional_extensionality. tauto. }
-       rewrite hh.
-       set_simpl.
-       reflexivity.
-    ++ exists nil.
-       cbn. 
-       set_crunch.
-       unfold constrain_ne,In in H0.
-       have hh: ((x ≈ ⟨ Int 0 ⟩) ρ) = False.
-       { unfold constrain_eq. 
-         eapply propositional_extensionality. tauto. }
-       rewrite hh. 
-       set_simpl.
-       eapply in_singleton.
-       auto.
-Qed. *)
-
-(* one { 0 | 1 } = [ {{ r = 0 }} ]     *)
-(* one { x = 0 } = [ {{ r = x = 0 }} ] *)
-(* one { x = 0 | x = 1 } = [ {{ r=x=0 }} union {{r=x=1}} ] *)
-
-Definition D0 : ENV := r ≈ ⟨ Int 0 ⟩.
-Definition D1 : ENV := r ≈ ⟨ Int 1 ⟩.
-Definition Dx v : ENV := x ≈ ⟨ v ⟩ ∩ r ≈ ⟨ v ⟩.
-
-
-Lemma extract_D0 : 
-  extract D0 = ⌈ ( Int 0, Total_set ) ⌉. 
-Admitted.
-Lemma extract_D1 :
-  extract D1 = ⌈ (Int 1 , Total_set) ⌉.
-Admitted.
-
-Lemma ONE_example1 : ONE [ D0 ; D1 ] = D0.
-Proof.
-  unfold ONE.
-  apply set_extensionality. intros ρ.
-  unfold consistent_results, In.
-  unfold fmap, Functor_list,ListDef.map.
-  rewrite extract_D0. rewrite extract_D1.
-  set_simpl.
-  unfold squash_pick.
-  unfold Head.
-  split.
-  + intros h.
-    inv h.
-    inv H.
-Admitted.
-(*    inv H0. 
-    unfold D0, constrain_eq. 
-    autorewrite with set_simpl in H1. inv H1.
-  + unfold D0. 
-    intro h. inv h.
-    exists [ Int 0 ; Int 1].
-    rewrite H0.
-    split.
-    cbn.
-    set_simpl.
-    eapply in_singleton. cbn.
-    eapply in_singleton.
-Qed.
-*)
-
-Lemma ONE_example2 : 
-  ONE [ Dx (Int 0) ] = Dx (Int 0).
-Admitted.
-
-Lemma bind_when {A B} ϕ (s : P A) (k : A -> P B) : 
-  (bind (when ϕ s) k) = (⟨ϕ⟩ ∩ (bind s k)).
-Proof.
-Admitted.
-
-Lemma If3_when_ret {A B} (k : A) ϕ (s2 s3 : P B): 
-  If3 (when ϕ (ret k)) s2 s3 = ((⟨ϕ⟩ ∩ s2) ∪ (⟨not ϕ⟩ ∩ s3)).
-Admitted.
-
-Lemma ONE_example3 : 
-  ONE [ Dx (Int 0) ; Dx (Int 1) ] = (Dx (Int 0) ∪ Dx (Int 1)).
-Proof.
-  unfold ONE, Dx, consistent_results.
-  apply set_extensionality. intros ρ.
-  unfold In.
-  unfold fmap, Functor_list, List.map.
-  repeat rewrite extract_example.
-  set_simpl.
-  split.
-  + intros h. set_crunch.
-    unfold Head, squash_pick in h.
-    cbn in h.
-Admitted.    
-
-
-Lemma ALL_two_example :
-  ALL (ret (r ≈ ⟨Int 0⟩ ∪ (r ≈ ⟨Int 1⟩))) = 
-      (r ≈ ⟨mkTup [Int 0]⟩ ∪ (r ≈ ⟨mkTup [Int 1]⟩)).
-  apply set_extensionality. intros ρ.
-  set_simpl.
-  unfold ALL.
-  unfold In.
-  list_simpl.
-Admitted.
-(*
-  rewrite extract_two.
-  rewrite bind_union.
-  repeat rewrite bind_ret_l.
-  replace (Total_set ρ) with True; try easy.
-  set_simpl.
-  rewrite squash_pick_two_example.
-  split.
-  + intro h. crunch.
-    inv H; inv H1. left; auto. right; auto.
-  + intro h. inv h.
-    exists [Int 0]. split; auto. left. eauto with sets.
-    exists [Int 1]. split; auto. right; eauto with sets.
-Qed.
-
-
-
-
-Lemma conflict_example : 
-  ALL2 [ x ≈ ⟨ Int 0 ⟩ ∩ r ≈ ⟨ Int 0 ⟩ ; 
-         x ≈ ⟨ Int 1 ⟩ ∩ r ≈ ⟨ Int 1 ⟩ ]
-   = (((x ≈ ⟨ Int 0 ⟩) ∩ (r ≈ ⟨ mkTup [Int 0] ⟩))
-   ∪ ((x ≈ ⟨ Int 1 ⟩) ∩ (r ≈ ⟨ mkTup [Int 1] ⟩))
-   ∪ ((x ≉ ⟨ Int 0 ⟩) ∩ x ≉ ⟨ Int 1 ⟩ ∩ (r ≈ ⟨ mkTup []⟩))).
-Admitted.  
-
-
-Lemma squash_irr_ALL (s : list ENV) : 
-  ALL2 s = ALL2 (squash s).
-Proof.
-  unfold ALL2.
-  eapply set_extensionality. intros ρ.
-  unfold In.
-  split.
-  + intro h. crunch.
-    exists x0. split; auto.
-Abort.
-    
-
-
-
-(* Ed[ e1; r=<> ] = [ hide(r) D1 ∩ {{ r=<> }} | D1 <- E[e1] ] *)
-Lemma part1 e1 : E (e1 :>: r :=: mini.Array []) = 
-        List.map (fun D1 => hide_r D1 ∩ (r ≈ ⟨mkTup []⟩)) (E e1).
-Proof.
-  cbn.
-  unfold hide_r. unfold hide_list. unfold UNIFY.
-  list_simpl.
-  set_simpl.
-Admitted.
-
-(*
-Ed[ (e1; r=<>) | r=0 ] = [ hide_r D1 \cap {{r=<>}} | D1 <- E[e1] ] ++ [ {{r=0}} ] 
-*)
-Lemma part2 e1 : E ( (e1 :>: r :=: mini.Array []) :|: r :=: 0) = 
-                fmap (fun D1 => hide_r D1 ∩ (r ≈ ⟨mkTup []⟩)) (E e1) ++ [ r ≈ ⟨Int 0⟩ ].
-rewrite E_Choice. 
-rewrite part1.
-cbn. set_simpl. done.
-Qed.
-
-(* ---- y = one{ (e1; z=<>) | z=0}@z -------------
-  Ed[ y = one{(e1; z=<>) | z=0}@z ]
-
-= [ { rho | v =<>,  
-      if rho ∈ UNIONLIST (map hide(z) E[e1])   # UNIONLIST :: [ENV] -> ENV, union them all
-               = 0,   otherwise
-     , rho y = v } ]
-*)
-
-
-Definition UNIONLIST : list ENV -> ENV := 
-  List.fold_right Union ∅.
-
-(* SCW this is NOT true. These are only true up to squashing. *)
-Lemma disjoint_append (S1 S2 S3 : ENV) : 
- [(S1 ∩ S2) ∪ (Total_set - S1 ∩ S3)] = [S1 ∩ S2] ++ [Total_set - S1 ∩ S3].
-Proof.
-  rewrite distrib_union_l.
-Abort.
-
-Definition if2 (ϕ1 : Prop) (ϕ3 : Prop) := 
-  (~ ϕ1 /\ ϕ3).
-
-Definition if3 (ϕ1 : Prop) (ϕ2 : Prop) (ϕ3 : Prop) := 
-  (ϕ1 /\ ϕ2) \/ (~ ϕ1 /\ ϕ3).
-
-Lemma if3_rhoIn (S1 S2 S3 : ENV) :
-  [ (fun ρ => if3 (ρ ∈ S1) (ρ ∈ S2) (ρ ∈ S3)) ] = 
-  [(S1 ∩ S2) ∪ (Total_set - S1 ∩ S3)].
-Proof.
-  unfold if3.
-  replace (fun ρ : env => ρ ∈ S1 /\ ρ ∈ S2 \/ ~ ρ ∈ S1 /\ ρ ∈ S3) with 
-          ((fun ρ => ρ ∈ S1 /\ ρ ∈ S2) ∪ (fun ρ => ~ ρ ∈ S1 /\ ρ ∈ S3)).
-  2: { set_ext ρ. rewrite in_union. intuition. }
-  replace (fun ρ => ρ ∈ S1 /\ ρ ∈ S2) with (S1 ∩ S2).
-  2: { set_ext ρ. rewrite in_intersection. intuition. inv H. auto. inv H. auto. } 
-  replace (fun ρ => ~ ρ ∈ S1 /\ ρ ∈ S3) with (Total_set - S1 ∩ S3).
-  2: { set_ext ρ. rewrite in_intersection. unfold In.
-       intuition. inv H0. done. unfold Total_set, Setminus. intuition. }
-  done.
-Qed.
-
-Lemma squash_pick_app : 
-  forall xs ys, squash_pick (xs ++ ys) = 
-             xs' ⭅ (squash_pick xs) ;; 
-             ys' ⭅ (squash_pick ys) ;; 
-             ⌈ xs' ++ ys' ⌉ .
-Proof. 
-  induction xs.
-  + intros ys. cbn. 
-    set_simpl.
-    reflexivity.
-  + intros ys.
-    cbn.
-    have h: ((Inhabited a) \/ (a = ∅)). admit.
-    inv h.
-    ++ repeat rewrite If3_nonempty; auto.
-       rewrite IHxs.
-       unfold Cons.
-       set_simpl.
-       f_equal.
-       apply functional_extensionality. intro v.
-       set_simpl.
-       f_equal.
-       apply functional_extensionality. intro vs.
-       rewrite Sets.bind_bind.
-       rewrite Sets.bind_singleton_l.
-       f_equal.
-       apply functional_extensionality. intro ws.
-       set_simpl.
-       done.
-    ++ repeat rewrite If3_empty; auto.
-Admitted.
-
-
-
-
-Lemma list_map_singleton {A B} (f:A -> B)(v:A) : 
-  List.map f [v] = [f v].
-Proof. auto. Qed.
-
-
-
-(* = 
-   Ed[ y = one{(e1; z=<>) | z=0}@z ]
-   = [ { rho | v  = tup[],  if rho ∈ UNIONLIST (map hide(z) E[e1]) 
-                  = 0,      otherwise
-             , rho y = v } ]
-*)
-
-Lemma if3_union: forall (S1 S1' : Prop) (S2 S3 : Prop),  
-                if3 (S1 \/ S1') S2 S3 = if3 S1 S2 (if3 S1' S2 S3).
-Proof.
- intros. unfold if3. 
- apply propositional_extensionality. tauto. Qed.
-
-Lemma part3 e1 : 
-    E (y :=: mini.One ((e1 :>: r :=: mini.Array []) :|: r :=: 0)) = 
-      let GOOD := UNIONLIST (List.map hide_r (E e1)) in
-      [ (GOOD ∩ (r ≈ y ≈ ⟨mkTup []⟩)) 
-      ∪ ((Total_set - GOOD) ∩ (r ≈ y ≈ ⟨Int 0⟩)) ].
-Proof.
-  rewrite E_Unify.
-  rewrite E_One.
-  rewrite part2.
-  rewrite hide_nothing.
-  rewrite E_Var.
-  unfold UNIFY.
-  list_simpl.
-
-  remember (fmap (fun D2 : ENV => hide_r D2 ∩ r ≈ ⟨ mkTup [] ⟩) (E e1) ++ [r ≈ ⟨ Int 0 ⟩]) as Δs.
-
-  rewrite <- if3_rhoIn.
-  remember (UNIONLIST (List.map hide_r (E e1))) as GOOD.
-
-  unfold ONE.
-
-  f_equal.
-  set_ext ρ. rewrite in_intersection. 
-
-  unfold In. 
-  remember  (List.map (consistent_results ρ) Δs) as S.
-  rewrite HeqΔs in HeqS.
-  unfold fmap, Functor_list in HeqS.
-  rewrite List.map_app in HeqS.
-  rewrite List.map_map in HeqS.
-  rewrite list_map_singleton in HeqS.
-  unfold consistent_results in HeqS.
-  rewrite extract_one in HeqS.
-  set_simpl in HeqS.
-  rewrite when_is_true in HeqS; [unfold Total_set;done|].
-
-  replace (fun x : ENV => x0 ⭅ extract (hide_r x ∩ r ≈ ⟨ mkTup [] ⟩);; 
-                       (let (v, Δ') := x0 in when (ρ ∈ Δ') (⌈v⌉)))
-     with (fun x : ENV => when (ρ ∈ hide_r x) (⌈mkTup []⌉)) 
-  in HeqS.
-  2: { 
-    apply functional_extensionality. intro Δ1.
-    unfold extract.
-    admit.
-  } 
-  subst.
-  rewrite squash_pick_app.
-
-  cbn.
-  rewrite If3_nonempty. econstructor;econstructor; eauto.
-  unfold Cons. set_simpl.
-  
-  split.
-  + intros h. crunch. 
-    rewrite H in H0. 
-    unfold Head in H0. 
-    set_simpl in H0.
-    inv H0; crunch.
-    inv H1; crunch.
-    set_simpl in H1.
-    destruct x0. 
-    ++ (* squash_pick fails *) 
-      inv H1.
-      cbn in H2. inv H2.
-
-       right. split; auto. 
-       2: { unfold constrain_eq. split. unfoldIn. done.
-            unfoldIn. done. }
-       intro h.
-
-       remember (E e1) as VS.
-       move: H0 h.
-       clear.
-       (* need to prove that it fails *)
-       move: ρ.
-       induction VS; intro ρ.
-       - cbn. done.
-       - intros. 
-         replace (a :: VS) with ([a] ++ VS) in H0. 2: { auto. } 
-         rewrite List.map_app in H0.
-         rewrite squash_pick_app in H0.
-         inv H0; crunch.
-         rewrite List.map_singleton in H.
-         cbn in H.
-         inv H0; crunch.
-         destruct x0. 2: { inv H1. } 
-         destruct x1. 2: { inv H1. } 
-         cbn in h. inv h.
-         -- rewrite when_is_true in H; auto.
-            rewrite If3_nonempty in H. econstructor; econstructor; eauto.
-            unfold Cons in H.
-            autorewrite with set_simpl in H.
-            inv H.
-         -- apply IHVS in H0. done. auto.
-    ++ (* squash pick succeeds *)
-      inv H1. clear H3.
-      remember (E e1) as VS.
-      clear HeqVS.
-      cbn in H2. inv H2.
-      induction VS as [|W WS].
-      - inv H0.
-      - cbn.
-        cbn in H0.
-        have CL: (ρ ∈ hide_r W) \/ ~(ρ ∈ hide_r W). admit.
-        destruct CL.
-        -- (* first one works *) 
-          clear IHWS.
-          rewrite when_is_true in H0; auto.
-          rewrite If3_nonempty in H0. econstructor; econstructor; eauto.
-          unfold Cons in H0.
-          set_simpl in H0.
-          inv H0; crunch.
-          inv H0; crunch.
-          clear H2.
-
-          replace ((hide_r W ∪ UNIONLIST (ListDef.map hide_r WS)) ρ) with
-            ((ρ ∈ hide_r W) \/ (ρ ∈ UNIONLIST (ListDef.map hide_r WS))). 2: { unfold In. admit. } 
-                                                                      
-          rewrite if3_union.
-          unfold if3. left. split. auto. split; eauto. 
-          rewrite H4. unfold constrain_eq. unfold In. done.
-      -- (* first one doesn't *)
-        rewrite when_is_false in H0; auto.
-        autorewrite with set_simpl in H0.
-        move: (IHWS H0) => ih. clear IHWS H0.
-        replace ((hide_r W ∪ UNIONLIST (ListDef.map hide_r WS)) ρ) with
-            ((ρ ∈ hide_r W) \/ (ρ ∈ UNIONLIST (ListDef.map hide_r WS))). 2: { admit. } 
-        rewrite if3_union.
-        unfold if3.
-        right.
-        split. auto.
-        unfold if3 in ih.
-        inv ih; crunch. left. split. auto. auto.
-        right. split. auto. auto.
- + intro h.
-   unfold if3 in h.
-   destruct h.
-   ++ (* ρ in UNIONLIST (E e1 \ r) *)
-     crunch.
-     inv H0. inv H1. done.
-     inv H0. inv H1. inv H2.
-     unfold Head.
-     set_simpl.
-Admitted.
-
-(* y = one{ (e1; z=<>) | z=0}@z; (y=⟨⟩; e2) | (y=0; e3)  
-  [ GOOD ⋂ {{y=<>}} ⋂ D | D ∈ Ed[e2] ] ++
-  [ BAD ⋂ {{y=0}}   ⋂ D  | D ∈ Ed[e3] ]
-*)
-
-Lemma UNIONLIST_hide VS s :
-  UNIONLIST (VS [\] s) = ((UNIONLIST VS) \ s).
-induction VS.
-cbn. set_simpl. done.
-cbn. set_simpl. f_equal.
-auto.
-Qed.
-
-Lemma part4 e1 e2 e3 : 
-  E (y :=: mini.One (e1 :>: r :=: mini.Array [] :|: r :=: 0) 
-       :>: 
-    ((y :=: mini.Array [] :>: e2) :|: (y :=: 0 :>: e3))) = 
-  let GOOD := UNIONLIST (List.map hide_r (E e1)) in
-  let BAD  := Total_set - GOOD in 
-  (List.map (fun D => GOOD ∩ (y ≈ ⟨mkTup []⟩) ∩ D) (E e2)) ++
-  (List.map (fun D => BAD  ∩ (y ≈ ⟨Int 0⟩) ∩ D) (E e3)).
-Proof.
-  rewrite E_Seq.
-  rewrite part3.
-  rewrite E_Choice.
-  repeat rewrite E_Seq.
-  repeat rewrite E_Unify.
-  repeat rewrite E_Var.
-  cbn.
-  remember (UNIONLIST (ListDef.map hide_r (E e1))) as GOOD.
-  remember (Total_set - GOOD) as BAD.
-  repeat rewrite flat_map_map.
-  repeat rewrite List.app_nil_r.
-  repeat rewrite List.map_app.
-  repeat rewrite List.map_map.
-  f_equal.
-  - f_equal.
-    apply functional_extensionality. intro D.
-    set_simpl.
-    set_ext ρ.
-    split.
-    ++ set_simpl.
-       intros [h1 h2].
-       inv h2. inv H. inv H1. inv H. inv H3. inv H1.
-       have NI: ~ Scope.In y ⟅ r ⟆. { admit. }
-       move: (H2 y ltac:(eauto))=> NY.
-       repeat split; try congruence.
-       inv h1.
-       -- unfold hide in H. inv H. 
-          inv H1.
-          inv H.
-          unfold constrain_eq in H6. inv H6. inv H. inv H7.
-          rewrite UNIONLIST_hide in H1. inv H1. crunch.
-          rewrite UNIONLIST_hide. unfold hide.
-          exists x2. split; auto. intros z zIn. rewrite H5; auto.
-       -- unfold hide in H. inv H. crunch.
-          inv H. unfold constrain_eq in H6.
-          inv H6. inv H. inv H7.
-          rewrite <- H1 in H6; auto.
-          rewrite H2 in H6; auto.
-          rewrite <- H3 in H6.
-          rewrite H4 in H6.
-          inv H6.
-    ++ set_simpl. 
-       intro h. inv h. inv H0.
-       split.
-       left.
-       rewrite  UNIONLIST_hide.
-       unfold hide. unfoldIn.
-       rewrite UNIONLIST_hide in H.
-       unfold hide in H. destruct H as [ρ' H].
-       inv H.
-       exists (r |-> mkTup [], ρ). repeat split.
-Admitted.
-
-End DLS.
-
-(*
-Module D2LS.
-
-Fixpoint E (e : mini.Expr) : list ENV := 
-
-  let B (e : mini.Expr) :list ENV := 
-    Δ <- E e ;; [Δ \ mini.I e] 
-  in
-  let V (e : mini.Expr) : list (P (value * ENV)) := 
-    Δ <- B e ;; [extract Δ] 
-  in
-
-  match e with 
-  | mini.DefineV _ => [ Total_set ]
-
-  | mini.Unify (mini.Var z) (mini.Var w) => 
-      [ z ≈ evalA (mini.Var w) ]
-
-  | mini.Unify (mini.Var z) (mini.Lit w) => [ r ≈ evalA (mini.Lit w) ]
-(*   | mini.EPrim _ => [ r ≈ evalA e ]
-  | mini.Array es =>  [ r ≈ evalA e ] *)
-
-  | mini.Fail => []  
-
-  | mini.Choice e1 e2 => E e1 ++ E e2
-
-  | mini.Seq e1 e2 => 
-      (E e1 * E e2) 
-
-
-  | mini.Unify (mini.Var z) (mini.ApplyD a1 a2) => 
-      APP e1 e2
-
-  | mini.If3 a b c =>  []
-
-  | mini.All a => 
-      [ ALL (E a) \ mini.I a ] 
-
-  | mini.One a => 
-      [ ONE (E a) \ mini.I a ]
-
-  (* TODO: functions *)
-
-  | _ => [ ] 
-  end.
-
-
-End D2LS.
-*)
-
-(* ----------- dest passing style Fig 20 ----------------- *)
-
+(* ----------- dest passing style - sets of lists of ENV -------------- *)
+(* TODO: complete this definition *)
 Module DSLS.
 
 Definition map2 {A B} : (A -> B) -> (P (list A)) -> (P (list B)) := 
-  fun f => fmap (fmap f).
+  fun f => Sets.map (List.map f).
 
 Fixpoint E (e : mini.Expr) : P (list ENV) := 
 
   let B (e : mini.Expr) : P (list ENV)  :=
-    List.map (fmap (hide (mini.I e))) (E e)
+    Sets.map (hide_list (mini.I e)) (E e) 
   in
 
   match e with 
@@ -1255,11 +524,21 @@ Fixpoint E (e : mini.Expr) : P (list ENV) :=
 
   | mini.Fail => ⌈ FAIL ⌉
 
-  | mini.Choice e1 e2 => List.map CHOICE (B e1) <*> B e2
+  | mini.Choice e1 e2 => 
+      D1 ⭅ E e1 ;;
+      D2 ⭅ E e2 ;;
+      ⌈ CHOICE D1 D2 ⌉
 
-  | mini.Seq e1 e2 => SEQ <$> E e1 <*> E e2
+  | mini.Seq e1 e2 => 
+      D1 ⭅ E e1 ;;
+      D2 ⭅ E e2 ;;
+      ⌈ SEQ D1 D2 ⌉
 
-  | mini.Unify e1 e2 => UNIFY <$> E e1 <*> E e2
+
+  | mini.Unify e1 e2 => 
+      D1 ⭅ E e1 ;;
+      D2 ⭅ E e2 ;;
+      ⌈ D1 * D2 ⌉
 (* 
   | mini.All e1 => (fun x => [ ALL x ]) <$> (B e1)
 *)
@@ -1271,114 +550,30 @@ Fixpoint E (e : mini.Expr) : P (list ENV) :=
 
   end.
 
-Module DSLS.
-
-(* ---------------------------------------------------- *)
-
-
-Definition x : Ident := mini.Test.x.
-
-
-(* { x:=1; x }  *)
-Lemma t2 : 
-  [ ⌈r |-> Int 1⌉ ] ∈ E mini.Test.t2.
-Proof.
-  unfold mini.Test.t2.
-  exists [ ⌈r |-> Int 1, mini.Test.x |-> Int 1⌉ ].
-Admitted.
-(*
-  split.
-  - admit.
-  - cbn.
-    eexists.
-    split.
-    eexists.
-    split; eapply in_singleton.
-    eexists.
-    repeat split.
-    2: {  rewrite SEQ_SUCCEED_X. eapply in_singleton. }    
-    eexists.
-    split.
-    eexists.
-    eexists.
-    eexists.
-    repeat split.
-    eexists. split.
-    eapply in_singleton.
-    eapply in_singleton.
-    eexists.
-    split.
-    eapply in_singleton.
-    eapply in_singleton.
-    eapply in_singleton.
-    eexists.
-    split.
-    eapply in_singleton.
-    unfold SEQ, UNIFY, hide.
-    cbn.
-    eapply in_singleton'.
-    f_equal.
-    eapply Extensionality_Ensembles.
-    split.
-    + intros x xIn. inversion xIn. 
-      split.
-      ++ unfold hide. cbv. 
-         exists x. subst x.
-         split. split. cbv. auto.
-         cbv. auto.
-         intros x nIn.
-         destruct x eqn:EX. cbn. auto.
-         destruct n eqn:EN. cbn. auto.
-         reflexivity.
-         
-      ++ unfold constrain.
-         cbv. auto.
-    + intros x xIn. inversion xIn. clear xIn H1 x0.
-      destruct H as [y [h1 h2]].
-      unfold constrain in *.
-      inversion H0. clear H0.
-      inversion h1. inversion H. inversion H0. clear h1 H H0. subst.
-      have NIN: ~ Scope.In mini.Test.x (Scope.singleton r). admit.
-      move: (h2 mini.Test.x NIN) => h3.
-      eapply in_singleton'.
-      symmetry.
-      eapply extend_equal. congruence.
-      intros z yNE. 
-      cbv.
-      destruct z eqn:HZ. cbv in yNE. done.
-      destruct n eqn:HN. subst.
-      unfold mini.Test.x in *.
-      unfold r,mini.Test.r in *.
-      rewrite h3. auto.
-Admitted.      
-*)      
-
 End DSLS.
-
-
-(* -------------------------------------------------------- *)
-(* -------------------------------------------------------- *)
-(* -------------------------------------------------------- *)
 
 (* ------------------------------------------------------ *)
 (* ------  Fig 15 E-LV (uses dodgy union) --------------- *)
 
 Module ELV.
 
+Definition Snoc (VS : VAL) (V : VAL) : VAL := 
+  vs ⭅ VS ;; v ⭅ V ;; ⌈ Dom.snoc vs v ⌉.
+
 Definition ALL (VS : list VAL) : VAL := 
-  squash_fold_left (liftM2 snoc) VS (ret (mkTup empty)).
+  squash_fold_left Snoc VS ⌈ mkTup [] ⌉ .
 
 Fixpoint E (e :mini.Expr) (ρ:env) : list VAL := 
   
   let B (e : mini.Expr) (ρ : env) : list VAL  := 
     DODGY_UNIONS
-      (ρ' <- X e ρ ;; ret (E e ρ')) 
+      (ρ' ⭅ X e ρ ;; ⌈ E e ρ' ⌉) 
     in
 
   let R (e : mini.Expr) ρ : ENV := 
-    ρ' <- X e ρ ;; 
-    when (E e ρ' <> empty) 
-    (ret ρ')
+    ρ' ⭅ X e ρ ;; 
+    when (E e ρ' <> []) 
+    ⌈ ρ' ⌉
   in
 
   match e with 
@@ -1409,7 +604,7 @@ Fixpoint E (e :mini.Expr) (ρ:env) : list VAL :=
       if is_Empty_set Δ then
         B e2 ρ
       else
-        DODGY_UNIONS ( ρ' <- Δ ;; ⌈ B e2 ρ' ⌉ )
+        DODGY_UNIONS ( ρ' ⭅ Δ ;; ⌈ B e2 ρ' ⌉ )
 
   (* TODO: functions, one *)      
 
@@ -1423,87 +618,7 @@ End ELV.
 
 
 (* ------------------------------------------------------ *)
-(* ------  E-LV (doesn't use dodgy union) --------------- *)
-
-Module NonDodgyELV.
-
-Definition ALL (VS : list VAL) : VAL := 
-  List.fold_left (liftM2 snoc) VS ⌈ mkTup [] ⌉.
-
-Fixpoint E (e :mini.Expr) (ρ:env) : P (list VAL) := 
-  
-  let B (e : mini.Expr) (ρ : env) : P (list VAL)  := 
-      (ρ' <- X e ρ ;; E e ρ' ) 
-    in
-
-(*
-  let R (e : mini.Expr) ρ : ENV := 
-    ρ' <- X e ρ ;; 
-    when (E e ρ' <> []) 
-    ⌈ ρ' ⌉
-  in
-*)
-
-  match e with 
-
-  | mini.Block e =>  B e ρ
-
-  | mini.Var _ => ⌈ [ ⌈evalA e ρ⌉ ] ⌉
-  | mini.Lit _ => ⌈[ ⌈evalA e ρ⌉ ] ⌉
-  | mini.EPrim _ => ⌈[ ⌈evalA e ρ⌉ ] ⌉
-  | mini.Array es =>  ⌈ [ ⌈evalA e ρ⌉ ] ⌉
-
-  | mini.DefineV _ => ⌈ [ ⌈ mkTup[] ⌉ ] ⌉
-
-  | mini.ApplyD e1 e2 => ⌈apply (evalA e1 ρ) (evalA e2 ρ) ⌉
-
-  | mini.Fail =>  ⌈[]⌉
-
-  | mini.Choice e1 e2 => CHOICE <$> (B e1 ρ) <*> (B e2 ρ)
-
-  | mini.Unify e1 e2 => UNIFY <$> (E e1 ρ) <*> (E e2 ρ)
-
-  | mini.Seq e1 e2 =>  IF2 <$> (E e1 ρ) <*> (E e2 ρ)
-
-  | mini.All e1 =>  
-      vs <- B e1 ρ ;;
-      ⌈ [ ALL vs ] ⌉
-
-(*
-  | mini.If3 e1 e2 e3 => 
-      let Δ  : ENV := R e1 ρ in
-      if is_Empty_set Δ then
-        B e2 ρ
-      else
-        DODGY_UNIONS ( ρ' <- Δ ;; ⌈ B e2 ρ' ⌉ )
-*)
-
-  (* TODO: functions, one *)      
-
-  | mini.Fun q eff i e1 (y,h,x) e2 =>  ∅
-  | _ => ∅
-
-  end.
-
-
-Definition t := (x :=: common.Int 0).
-
-Example example1 :
-  E t (x |-> Int 0) ≃ ⌈ [ ⌈Int 0⌉ ] ⌉.
-Admitted.
-
-Example example2 :
-  E t (x |-> Int 1) ≃ ⌈ [ ] ⌉.
-cbn.
-split.
-+ intros x xIn.
-Admitted.
-
-End NonDodgyELV.
-
-
-(* ------------------------------------------------------ *)
-(* ------  Sets of lists of values (nondodgy)------------ *)
+(* ------  Sets of lists of values ---------------------- *)
 
 Module ESL.
 
@@ -1515,26 +630,18 @@ Definition apply (f : value) (v : value) : list value :=
   | Dom.Fun hs => 
       h <- hs ;;
       match (PFun.apply_opt _ _ Value.eqb h v) with 
-      | Some w => ret w
-      | None => empty
+      | Some w => [w]
+      | None => []
       end
-  | _ => empty
+  | _ => []
   end.
 
 
 Fixpoint E (e :mini.Expr) (ρ:env) : P (list value) := 
   
   let B (e : mini.Expr) (ρ : env) : P (list value)  := 
-      (ρ' <- X e ρ ;; E e ρ' ) 
+      (ρ' ⭅ X e ρ ;; E e ρ' ) 
     in
-
-(*
-  let R (e : mini.Expr) ρ : ENV := 
-    ρ' <- X e ρ ;; 
-    when (E e ρ' <> []) 
-    ⌈ ρ' ⌉
-  in
-*)
 
   match e with 
 
@@ -1551,31 +658,13 @@ Fixpoint E (e :mini.Expr) (ρ:env) : P (list value) :=
 
   | mini.Fail =>  ⌈[]⌉
 
-  | mini.Choice e1 e2 => CHOICE <$> (B e1 ρ) <*> (B e2 ρ)
+  | mini.Choice e1 e2 => ∅
 
-  | mini.Unify e1 e2 => 
-      vs1 <- (E e1 ρ) ;;  (* list in first set *)
-      vs2 <- (E e2 ρ) ;;  (* list in second set *)
-      let unify (vs1 : list value) (vs2 : list value) : list value :=
-        v1 <- vs1 ;;
-        v2 <- vs2 ;; 
-        if (Value.eqb v1 v2) then [v1] else []
-      in
-      (* need to return a set of lists *)
-      ⌈ unify vs1 vs2  ⌉
+  | mini.Unify e1 e2 => ∅
 
-  | mini.Seq e1 e2 =>  
-      vs1 <- (E e1 ρ) ;;  (* list in first set *)
-      vs2 <- (E e2 ρ) ;;  (* list in second set *)
-      let seq (vs1 : list value) (vs2 : list value) : list value :=
-        v1 <- vs1 ;; (* make sure vs1 is inhabited *)
-        vs2 
-      in
-      (* need to return a set of lists *)
-      ⌈ seq vs1 vs2  ⌉
-
+  | mini.Seq e1 e2 =>  ∅
   | mini.All e1 =>  
-      vs <- B e1 ρ ;;
+      vs ⭅ B e1 ρ ;;
       ⌈ [ ALL vs ] ⌉
 
   (* TODO: functions, one *)      
@@ -1585,20 +674,21 @@ Fixpoint E (e :mini.Expr) (ρ:env) : P (list value) :=
 
   end.
 
+End ESL.
 
 (* -------------------------------------------------------- *)
 
 Lemma Equiv1 (e : mini.Expr) (ρ : env) : 
   ELV.E e ρ = 
     Δ <- DLS.E e ;;
-    [ '(v, Δ') <- extract Δ ;;
+    [ '(v, Δ') ⭅ extract r Δ ;;
          when (ρ ∈ Δ') ⌈v⌉ ].
 Admitted.
 
 Lemma Equiv2 (e : mini.Expr) : 
   DLS.E e = 
     i <- allNums ;;
-    [ ρ <- Total_set ;;
+    [ ρ ⭅ Total_set ;;
       let VS := ELV.E e ρ in
       when (ρ r ∈ List.nth i VS ∅) 
       ⌈ ρ ⌉ ].
@@ -1606,172 +696,9 @@ Admitted.
 
 
 
-(* if((y=3) | (y=5)){y} else :false *)
+(* ----------------- ELV defined with a fixpoint ----------- *)
 
-Definition example_If3 := mini.If3 ((mini.Test.y :=: 3 ) :|: (mini.Test.y :=: 5)) mini.Test.y mini.Fail.
-
-Lemma hide_none ρ : hide Scope.empty ρ = ρ. Admitted.
-
-Example example : E example_If3 = [ r ≈ ⟨ 3 ⟩ ].
-Proof.
-  cbn.
-  repeat rewrite hide_none.
-  rewrite empty_Union.
-  rewrite hide_constraint.
-
-End NonDodgy.
-
-(* -------------- Squash ------------ *)
-
-
-(* Squashed VS WS holds when WS := filter (fun x => x <> ∅) VS
-
-   NOTE: We cannot define this as a function because results
-   in Type cannot depend on Prop. But this relation 
-   is total and functional.
-*)
-Inductive Squash {A} : list (P A) -> list (P A) -> Prop := 
-  | sq_nil : Squash nil nil 
-  | sq_consIn : forall x xs ys,
-    x <> ∅ ->
-    Squash xs ys -> 
-    Squash (cons x xs) (cons x ys)
-  | sq_consOut : forall x xs ys,
-    x = ∅ ->
-    Squash xs ys -> 
-    Squash (cons x xs) ys.
-
-(* A success is any list that contains at least one nonempty VAL *)
-Definition Succeeds (VS : P (list VAL)) : Prop :=
-  forall l, l ∈ VS -> exists v, v <> ∅ /\ List.In v l.
-
-Lemma Squash_functional {A} (VS : list (P A)) : forall WS1 WS2,
-      Squash VS WS1 -> Squash VS WS2 -> WS1 = WS2.
-Proof. 
-  induction VS; intros WS1 WS2 h1 h2; inversion h1; inversion h2; subst.
-  all: try done.
-  all: eauto.
-  - erewrite (IHVS ys ys0); auto.
-Qed.
-
-(* NOTE: Showing that Squash is functional requires classical reasoning. 
-   We need to know that 
-
-       forall any S, S = ∅ \/ S <> ∅
-
-   In order to prove this lemma:
-*)
-
-Lemma Squash_total {A} (decide_equality : forall (S:P A), S = ∅ \/ S <> ∅) 
-  : forall (VS : list (P A)), exists WS, Squash VS WS.
-Proof.
-  induction VS. exists nil. eapply sq_nil.
-  move: IHVS => [WS' IHWS'].
-  destruct (decide_equality a).
-  + exists WS'. eapply sq_consOut; auto.
-  + exists (a :: WS'). eapply sq_consIn; auto.
-Qed.
-
-(* The list is either empty, or the last element is inhabited. *)
-Definition NonEmptyTail {A} : list (P A) -> Prop := 
-  fun VS => 
-    match VS with 
-    | [] => True 
-    | _  => exists WS d, VS = WS ++ [d] /\ d <> ∅
-    end.
-
-Definition TailSquash {A} : list (P A) -> list (P A) -> Prop := 
-  fun VS WS => 
-    (exists n, VS = WS ++ List.repeat ∅ n) /\ NonEmptyTail WS.
-
-
-Lemma UNIONS_mem (ls : list (list VAL)) : (UNIONS (mem ls)) = ⌈ Pointwise_Unions ls ⌉.
-Proof.
-Admitted.
-
-
-
-Module NonDodgyELV.
-
-Fixpoint E (e : mini.Expr) (rho : env) : list VAL := 
-  
-  (* We can find the set of lists of VALs that result 
-     for any extension of rho.
-
-     But what do we do with this set? We don't want to 
-     pointwiseunion it.
-
-     We can fail if it is nonsingleton.
-   *)
-  let D (rho : env) (e : mini.Expr )  : list VAL :=
-    let output : P (list VAL) :=  
-         (rho' <- X e rho ;; E_e rho' e)  in
-
-  (* all extended environments that succeed when evaluating e *)
-  let R (rho : env) (e : mini.Expr) : ENV := 
-    rho' <- X e rho  ;;
-    VS <- E_e rho' e ;;
-    ⌈ rho' ⌉ in
-  
-  match e with 
-  | mini.Block e => D rho e
-
-  | mini.Var _ =>   ⌈[ ⌈evalA e rho⌉ ]⌉
-  | mini.Lit _ =>   ⌈[ ⌈evalA e rho⌉ ]⌉
-  | mini.EPrim _ => ⌈[ ⌈evalA e rho⌉ ]⌉                     
-  | mini.Array _ => ⌈[ ⌈evalA e rho⌉ ]⌉
-
-  | mini.DefineV x => ⌈[ ⌈mkTup nil⌉ ]⌉
-
-  | mini.Seq e1 e2 =>
-     VS1  <- E_e rho e1 ;;    (* outer set monad *)
-     VS1' <- Squash VS1 ;;
-     VS2  <- E_e rho e2 ;;  
-     pure (s1 <- VS1' ;; s2 <- VS2 ;; [s2] )  (* inner list monad *)
-
-  | mini.Unify e1 e2 => 
-     VS1 <- E_e rho e1 ;;
-     VS2 <- E_e rho e2 ;;
-     pure ( s1 <- VS1 ;; s2 <- VS2 ;; [s1 ∩ s2] )
-
-  | mini.Choice e1 e2 =>
-     VS1 <- D rho e1 ;;
-     VS2 <- D rho e2 ;;
-     pure (VS1 ++ VS2)
-
-  | mini.Fail => 
-      pure []
-
-  | mini.One e => 
-      VS1 <- E_e rho e ;;
-      VS2 <- Squash VS1 ;;
-      pure (take1 VS2)
-
-  | mini.All e => 
-      VS1 <- D rho e ;;
-      VS2 <- Squash VS1 ;;
-      pure [tups VS2]
-
-  | mini.If3 e1 e2 e3 =>
-      let Δ := R rho e1 in
-      TestEmpty Δ (D rho e3)
-        (UNIONS (rho' <- Δ ;; E_e rho' e2))
-  | _ => empty
-  end.
-
-End FixpointVersion.
-
-
-
-
-
-(* ----------------- version: fixpoint ----------- *)
-
-
-
-
-
-Module FixpointVersion.
+Module ESLV_Fixpoint.
 
 (* In this version, the denotation is defined as a fixpoint 
    over the syntax of miniverse expressions, taking an 
@@ -1810,12 +737,12 @@ Fixpoint E_e (rho : env) (e : mini.Expr) : P (list VAL) :=
      dodgy unioning the results together into a set 
      containing at most 1 result *)
   let D (rho : env) (e : mini.Expr )  : P (list VAL) :=
-    UNIONS (rho' <- X e rho ;; E_e rho' e ) in
+    (rho' ⭅ X e rho ;; E_e rho' e ) in
 
   (* all extended environments that succeed when evaluating e *)
   let R (rho : env) (e : mini.Expr) : ENV := 
-    rho' <- X e rho  ;;
-    VS <- E_e rho' e ;;
+    rho' ⭅ X e rho  ;;
+    VS ⭅ E_e rho' e ;;
     ⌈ rho' ⌉ in
   
   match e with 
@@ -1829,46 +756,48 @@ Fixpoint E_e (rho : env) (e : mini.Expr) : P (list VAL) :=
   | mini.DefineV x => ⌈[ ⌈mkTup nil⌉ ]⌉
 
   | mini.Seq e1 e2 =>
-     VS1  <- E_e rho e1 ;;    (* outer set monad *)
-     VS1' <- Squash VS1 ;;
-     VS2  <- E_e rho e2 ;;  
-     pure (s1 <- VS1' ;; s2 <- VS2 ;; [s2] )  (* inner list monad *)
+     VS1  ⭅ E_e rho e1 ;;    (* outer set monad *)
+     VS1' ⭅ Squash VS1 ;;
+     VS2  ⭅ E_e rho e2 ;;  
+     ⌈ (s1 <- VS1' ;; s2 <- VS2 ;; [s2]) ⌉  (* inner list monad *)
 
   | mini.Unify e1 e2 => 
-     VS1 <- E_e rho e1 ;;
-     VS2 <- E_e rho e2 ;;
-     pure ( s1 <- VS1 ;; s2 <- VS2 ;; [s1 ∩ s2] )
+     VS1 ⭅ E_e rho e1 ;;
+     VS2 ⭅ E_e rho e2 ;;
+     ⌈ ( s1 <- VS1 ;; s2 <- VS2 ;; [s1 ∩ s2]) ⌉
 
   | mini.Choice e1 e2 =>
-     VS1 <- D rho e1 ;;
-     VS2 <- D rho e2 ;;
-     pure (VS1 ++ VS2)
+     VS1 ⭅ D rho e1 ;;
+     VS2 ⭅ D rho e2 ;;
+     ⌈ (VS1 ++ VS2) ⌉
 
   | mini.Fail => 
-      pure []
+      ⌈ [] ⌉
 
   | mini.One e => 
-      VS1 <- E_e rho e ;;
-      VS2 <- Squash VS1 ;;
-      pure (take1 VS2)
+      VS1 ⭅ E_e rho e ;;
+      VS2 ⭅ Squash VS1 ;;
+      ⌈ take1 VS2 ⌉
 
   | mini.All e => 
-      VS1 <- D rho e ;;
-      VS2 <- Squash VS1 ;;
-      pure [tups VS2]
+      VS1 ⭅ D rho e ;;
+      VS2 ⭅ Squash VS1 ;;
+      ⌈ [tups VS2] ⌉
 
   | mini.If3 e1 e2 e3 =>
       let Δ := R rho e1 in
       TestEmpty Δ (D rho e3)
-        (UNIONS (rho' <- Δ ;; E_e rho' e2))
-  | _ => empty
+        (rho' ⭅ Δ ;; E_e rho' e2)
+  | _ => ∅
   end.
 
-End FixpointVersion.
+End ESLV_Fixpoint.
 
 
 (* ----------------- version two: Inductive relation ----------- *)
 
+(*
+Module ELV_Inductive.
 
 (* Type of denotation relation *)
 Definition D := forall (rho : env) (e : mini.Expr), (list VAL) -> Prop.
@@ -1884,7 +813,7 @@ Definition check (eval:D) (rho:env) (q:Aperture)
         exists V1, eval rho' e1 V1 /\
 
              (* evaluating e1 fails and applying h also fails *) 
-             (Squash V1 [] /\ exists V2, apply (rho h) v = V2 /\ Squash V2 []) 
+             (Squash V1 [] /\ exists (V2 : VAL), ESL.apply (rho h) v = V2 /\ Squash V2 []) 
               \/
 
              (* evaluating e1 produces a singleton value vx *)
@@ -2021,425 +950,7 @@ with eval_if (rho : env) : mini.Expr -> list VAL -> Prop :=
     eval_if rho (mini.If3 e1 e2 e3) VS
 .
 
-Definition eval_top t d := eval Env.empty t d.
-
-Lemma notIn_singleton {A}{v : A} : ~ List.In ∅ [⌈ v ⌉]. 
-Proof.
-  intro h. inversion h.  apply singleton_not_empty in H. done. inversion H.
-Qed.
-
-
-Lemma NonEmptyTail_nil {A} : @NonEmptyTail A [].
-done. Qed.
-Lemma NonEmptyTail_singleton {A}{v :A}: NonEmptyTail [ ⌈v⌉ ].
-cbn. exists nil. exists ⌈v⌉. cbv. split; auto; eapply singleton_not_empty. Qed.
-
-Lemma TailSquash_singleton {A} (v:A) VS : 
-  VS = [⌈ v ⌉] ->
-  TailSquash [⌈ v ⌉] VS.
-Proof. intros ->. unfold TailSquash. split. exists 0. cbn. auto.
-eapply NonEmptyTail_singleton; eauto. Qed.
-
-Lemma TailSquash_nil (VS : list VAL) : 
-  VS = nil ->
-  TailSquash [] VS.
-Proof. intros ->. unfold TailSquash. split. exists 0. cbn. auto.
-eapply NonEmptyTail_nil; eauto. Qed.
-
-Lemma TailSquash_empty (VS : list VAL) : 
-  VS = nil ->
-  TailSquash [∅] VS.
-Proof. intros ->. unfold TailSquash. split. exists 1. cbn. auto.
-eapply NonEmptyTail_nil; eauto. Qed.
-
-Lemma noEmptyInSquash : forall {A} (xs ys : list (P A)), Squash xs ys -> 
-                                   not (List.In ∅ ys).
-Proof.
-  induction 1; unfold not; intros. inversion H.
-  inversion H1. contradiction. contradiction. contradiction.
-Qed.
-
-Lemma Squash_singleton {A} (v:A) VS : 
-  VS = [⌈ v ⌉] ->
-  Squash [⌈ v ⌉] VS.
-Proof. intros ->. eapply sq_consIn; eauto using singleton_not_empty.
-       eapply sq_nil. Qed.
-
-Lemma Squash_nil (VS : list VAL) : 
-  VS = nil ->
-  Squash [] VS.
-Proof. intros ->. eapply sq_nil. Qed.
-
-Hint Resolve 
-  singleton_not_empty 
-  NonEmptyTail_nil 
-  NonEmptyTail_singleton 
-  notIn_singleton
-  TailSquash_singleton
-  TailSquash_nil
-  TailSquash_empty
-  Squash_singleton
-  Squash_nil
- :sets.
-
-Lemma Squash_singleton_invert {A} (v:A) VS : 
-  Squash [⌈ v ⌉] VS -> VS = [⌈ v ⌉].
-Proof. intro h. inversion h. subst. inversion H3. auto.
-subst. apply singleton_not_empty in H1. done. Qed.
-Lemma Squash_nil_invert {A} (VS : list (P A)) : 
-  Squash [] VS -> VS = [].
-Proof. intro h. inversion h. auto. Qed.
-Lemma Squash_empty_invert {A} (VS : list (P A)) : 
-  Squash [∅] VS -> VS = [].
-Proof. intro h. inversion h. done. inversion H3. done. Qed.
-
-
-Ltac ego := eauto with sets ; 
-            cbn ; 
-            try rewrite Intersection_same ;
-            try (rewrite Intersection_diff ; 
-                 [ intros ? ; discriminate| eauto with sets]) ;
-            eauto with sets.
-
-Ltac eeval1 := match goal with 
-              | [ |- eval ?env ?e ?VS ] =>
-                  econstructor ; eauto end.
-
-
-Ltac eeval := match goal with 
-              | [ |- eval ?env (mini.Seq _ _) ?VS ] =>
-                  econstructor ; 
-                  [ eeval | eauto with sets | eeval 
-                  | eauto with sets 
-                  | cbn ; eauto with sets ]
-              | [ |- eval ?env (mini.Unify _ _) ?VS ] =>
-                  econstructor ; [ eeval | eeval | ego ]
-              | [ |- eval ?env (mini.Var _) ?VS ] =>
-                  econstructor ; cbn ; eauto 
-              | [ |- eval ?env ?e ?VS ] =>
-                  econstructor ; eauto end.
-
-
-
-(* ----------------------- examples --------------- *)
-
-
-Lemma not_r : forall (x r : Ident), (SetoidList.InA eq x [r] -> False) -> Nat.eqb r x = false. Admitted.
-
-
-
-Lemma hide_constraint {i v} : (i ≈ fun _ => v) \ (Scope.singleton i) ≃ Total_set.
-split. 
-intros x xIn. cbv. auto.
-intros ρ ρIn. cbv.
-eexists.
-instantiate (1 := i |-> v, ρ).
-split. rewrite extend_lookup_same. auto.
-intros x NI. 
-apply not_r in NI. rewrite extend_lookup_diff; auto.
-Qed.
-
-Lemma hide_all s : (hide s Total_set) = Total_set.
-  eapply Extensionality_Ensembles.
-  split.
-  intros x xIn. cbv. auto.
-  intros x xIn. unfold hide.
-  exists x. split. auto.
-  intros y IH. auto.
-Qed.
-
-
-
-Lemma SEQ_SUCCEED_X X : SEQ SUCCEED X = X.
-  unfold SEQ, UNIFY, hide_list, SUCCEED.
-  cbn.
-  rewrite hide_all.
-  rewrite List.app_nil_r.
-  induction X.
-  - cbn. auto.
-  - cbn. f_equal.
-    eapply all_intersect.
-    auto.
-Qed.
-
-Example ex_ALL : 
-  (r |-> mkTup [Int 3;Int 4]) ∈ (ALL [ r ≈ ⟨3⟩;  r ≈ ⟨4⟩] ).
-cbn. exists ([Int 3; Int 4], Total_set).
-split; [exists (Int 3, Total_set);split|idtac]. 
-- cbv. extensionality ρ.
-  eapply propositional_extensionality.
-  split; try done. intro h.
-  exists (Env.extend r (Int 3) ρ). 
-  split. split. cbv. auto. cbv. auto.
-  intros x xIn. apply not_r in xIn. 
-  cbv. destruct x. done. done.
-- cbv.
-Admitted.
-
-
-Example first_example_none {A} : @first A  [ ∅ ] = ∅ .
-  eapply Extensionality_Ensembles. split.
-  - move => y yIn. 
-    unfold first in yIn. cbv in yIn.
-    inversion yIn; inversion H; subst; auto.
-  - move => y yIn. done.
-Qed.
-
-Example first_example {A} (x:A) : first  [ ∅ ; ∅ ; ⌈ x ⌉ ] = ⌈ x ⌉.
-Proof.
-  eapply Extensionality_Ensembles. split.
-  - move => y yIn. 
-    inversion yIn; inversion H; subst.
-    eapply not_Singleton_empty; eauto.
-    auto.
-  - move => y yIn.
-    right.
-    split. intro h. eapply not_Singleton_empty; eauto. auto.
-Qed.
-
-Example apply_tup0 x y : apply (mkTup [x;y]) (Int 0) = [ ⌈ x ⌉ ; ∅ ]. cbn. auto. Qed.
-Example apply_tup1 x y : apply (mkTup [x;y]) (Int 1) = [ ∅ ; ⌈ y ⌉ ]. cbn. auto. Qed.
-Example apply_add1 : apply Prim.add1 (Int 0) = [ ⌈ Int 1 ⌉ ]. cbn. auto. Qed.
-Example apply_isInt : apply Prim.isInt (Int 1) = [ ⌈ Int 1 ⌉ ]. cbn. auto. Qed.
-
-Example DODGY_UNIONS_ex : 
-  DODGY_UNIONS (⌈ [ ∅ ; ⌈ 3 ⌉ ] ⌉ ∪ ⌈ [ ⌈ 4 ⌉ ] ⌉) = 
-    [  ⌈ 4 ⌉ ; ⌈ 3 ⌉ ].
-Proof.
-  unfold DODGY_UNIONS, allNums. 
-  replace limitNum with 2.
-  cbn.
-  repeat rewrite map_union. repeat rewrite map_singleton.
-  cbn.
-  repeat rewrite -> UNION_union. 
-Admitted.  
-
-
-Module Test.
-
-Coercion Dom.Int : nat >-> value.
-
-(*   {y:=if(x=1){0|1}else{2|3}; x:=0|1; y}  =?= 2|0|3|1 *)
-
-Definition y := mini.Test.y.
-Definition x := mini.Test.x.
-
-Definition lennart := 
-  { y :=: mini.If3 (mini.Unify x 1) (0 :|: 1) (2 :|: 3) :>: 
-    x :=: (0 :|: 1)  :>:
-    y }.
-
-Lemma dodgy : eval Env.empty lennart 
-                ([ ⌈ Dom.Int 2 ⌉ ; ⌈ Dom.Int 0 ⌉ ; ⌈ Dom.Int 3 ⌉ ; ⌈ Dom.Int 1 ⌉ ]).
-Proof.
-  unfold lennart.
-  eeval.
-  instantiate (1 := 
-    (mem [ [ ⌈ Dom.Int 2 ⌉ ; ⌈ Dom.Int 0 ⌉ ; ⌈ Dom.Int 3 ⌉ ; ⌈ Dom.Int 1 ⌉ ] ;
-           [ ⌈ Dom.Int 2 ⌉ ; ⌈ Dom.Int 0 ⌉ ; ⌈ Dom.Int 3 ⌉ ; ⌈ Dom.Int 1 ⌉ ] ])).
-  intros WS WSIn.
-  apply mem_In in WSIn.
-  destruct WSIn.
-  - (* first option *)
-    exists ( (Env.extend y (Dom.Int 2) (Env.extend x (Dom.Int 1) Env.empty))).
-Admitted.
-
-
-Lemma t1 : eval_top mini.Test.t1 [ ⌈ Dom.Int 2 ⌉ ].
-Proof. unfold mini.Test.t1, eval_top. repeat eeval. Qed.
-
-
-(* { x:=1; x }  *)
-Lemma t2 : 
-  eval Env.empty mini.Test.t2 [ ⌈ Dom.Int 1 ⌉ ].
-Proof. unfold mini.Test.t2.
-       (* set up the block. *)
-       eeval1.
-       instantiate (1 := mem [ [ ⌈ Dom.Int 1 ⌉] ]).
-       intros WS WSIn.
-       2: { rewrite UNIONS_mem. cbn. eapply in_singleton. } 
-       apply mem_In in WSIn. cbn in WSIn.
-       destruct WSIn. 
-       - subst.
-         exists (mini.Test.x |-> Dom.Int 1 ).
-         split; auto.
-(*
-         ++ intros y.
-            destruct Scope.mem eqn:IN.
-            -- (* in new scope *) 
-              unfold mini.I in IN.
-              cbn in IN. fold Nat.compare in IN.
-              destruct Nat.compare eqn:CMP; try done.
-              apply PeanoNat.Nat.compare_eq in CMP. subst.
-              eexists. cbn. eauto. 
-            -- (* in old scope *)
-              unfold mini.I in IN.
-              cbn in IN. fold Nat.compare in IN.
-              destruct Nat.compare eqn:CMP; try done.
-              apply PeanoNat.Nat.compare_lt_iff in CMP.
-              admit.
-              admit.
-         ++ eeval.
-       - done. *)
-Admitted.
-
-
-
-(* No block here. *)
-(* x:=1; y:= if(x=2) then 0 else 3; y *)
-
-Lemma t7 : 
-  exists vx, exists vy, eval (Env.extend mini.Test.x vx (Env.extend mini.Test.y vy Env.empty)) mini.Test.t7 [ ⌈ Dom.Int 3 ⌉ ].
-Proof.  exists (Dom.Int 1). exists (Dom.Int 3).
-        unfold mini.Test.t7.
-        eapply eval_Seq.
-        - eeval.
-        - ego.
-        - eapply eval_Seq.
-          + eeval.
-          + ego.
-          + eapply eval_Seq.
-            -- eeval.
-            -- ego.
-            -- eapply eval_Unify.
-               ++ eeval.
-               ++ eeval1.
-                  +++ eapply eval_If3_false.
-                  --- intros rho' rho'X.
-                      unfold X, Ensembles.In in rho'X. 
-Admitted.
-(*
-                      move: (rho'X mini.Test.x) => [h _].
-                      cbn in h.
-                      specialize (h (Dom.Int 1) ltac:(auto)).                       
-                      eeval.
-                  --- eeval.
-               ++ ego.
-            -- ego.
-            -- ego.
-          + ego.
-          + ego.
-        - ego.
-        - ego.
-Qed.
-*)
-End Test.
-
-
-Module Theory.
-
-Lemma NonEmptyTail_UNIONS : 
-  forall V VV, 
-    UNIONS VV V -> 
-    (forall VS, VS ∈ VV -> NonEmptyTail VS) -> 
-    NonEmptyTail V.
-Proof.
-  intro V. induction V.
-  - intros.
-    unfold UNIONS in *.
-    unfold NonEmptyTail.
-    cbn. eauto with sets.
-  - intros VV VH U.    
-    unfold UNIONS in *.
-Admitted.
-
-Lemma NonEmptyTail_app {A} ( VS1 VS2 : list (P A)) : 
-  NonEmptyTail VS1 -> NonEmptyTail VS2 ->
-  NonEmptyTail (VS1 ++ VS2).
-Admitted.
-
-Fixpoint evalNonEmptyTail {e}{rho}{VS} (ev : eval rho e VS) : NonEmptyTail VS.
-  destruct ev; subst; eauto.
-  all: try eapply NonEmptyTail_singleton.
-  all: try solve [match goal with 
-    | [ H : TailSquash _ ?VS |- _ ] => move: H => [ _ h1 ] 
-    end; done].
-  - (* block *)
-    eapply NonEmptyTail_UNIONS; eauto.
-    intros V1 in1.
-    
-Admitted.
-
-(*
-Lemma evalNonEmptyTail : 
-  forall e rho VS, eval rho e VS -> NonEmptyTail VS.
-Proof.
-  induction 1.
-  all: subst.
-  all: auto.
-  all: try eapply NonEmptyTail_singleton.
-
-  (* true because we tail squashed *)
-  all: try solve [match goal with 
-    | [ H : TailSquash _ ?VS |- _ ] => move: H => [ _ h1 ] 
-    end; done].
-  - (* block *)
-
-  - (* choice *)
-    eapply NonEmptyTail_app; eauto.
-  - (* one *)
-    admit.
-  - (* all *)
-    admit.
-Admitted.
+End ELVInductive.
 *)
 
-End Theory.
 
-
-Module Rewrites.
-
-Ltac invert_eval := 
-  match goal with 
-  | [ H : eval ?rho (_ _) ?S |- _ ] => inversion H; subst; clear H 
-  | [ H : evalA ?rho (_ _) ?S |- _ ] => inversion H; subst; clear H 
-  | [ H : List.Forall2 (evalA _) (cons _ _) _ |- _ ] => 
-      inversion H; subst; clear H 
-  | [ H : List.Forall2 (evalA _) nil _ |- _ ] => 
-      inversion H; subst; clear H 
-  end.
-
-Lemma VarSwap : forall rho (x y : Ident) e, 
-    eval rho ((mini.Var x :=: mini.Var y) :>: e) ⊆
-    eval rho ((mini.Var y :=: mini.Var x) :>: e).
-Proof. 
-  intros.
-  intros VS vIn. unfold Ensembles.In in *.
-  invert_eval.
-  invert_eval.
-  invert_eval.
-  invert_eval.
-  cbn in H9.
-  eapply eval_Seq.
-Admitted.
-
-
-
-Lemma AppTup x rho v v0 v1: 
-  eval rho 
-  (mini.DefineV x :>: (mini.Var x :=: mini.Array [v0 ; v1])  :>: (mini.Var x :@: mini.Lit (common.Int v))) ⊆
-  eval rho (((mini.Lit (common.Int v) :=: mini.Lit (common.Int 0)) :>: v0) :|: ((mini.Lit (common.Int v) :=: mini.Lit (common.Int 1)) :>: v1)).
-Proof.
-  intros VS vIn. unfold Ensembles.In in *.
-  repeat invert_eval.
-  clear H4.
-  apply Squash_singleton_invert in H2. subst.
-Admitted.
-
-(*
-Lemma AppLam rho (x y :Ident) v e : 
-  eval rho 
-    (mini.DefineV y :>:
-       (mini.Var y :=: (mini.Fun Closed Succeeds x (mini.Var x) None e)) :>: 
-    (mini.ApplyD (mini.Var y) v)) ⊆
-  eval rho ((mini.DefineV x) :>: mini.Var x :=: v :>: e).
-Proof.
-  intros VS vIn. unfold Ensembles.In in *.
-  invert_eval.
-  invert_eval.
-  invert_eval.
-  invert_eval.
-  inversion H3. subst. clear H3.
-Admitted. *)
-
-End Rewrites.
