VerseRocq/verse/densem/examplesDLS.v
@@ -1,0 +1,934 @@
+Require Import Imports.
+
+From Stdlib Require Lists.List.
+From Stdlib Require Import Classes.EquivDec.
+Import ssreflect.
+
+From Stdlib Require Import Logic.PropExtensionality.
+From Stdlib Require Import Logic.FunctionalExtensionality.
+From Stdlib Require Import Sets.Classical_sets.
+
+Require Import syntax.common.
+Require syntax.mini.
+Require Import PFun.
+Require Import structures.Sets.
+Import structures.List.
+
+Require Import densem.Dom.
+Require Import densem.tenv.  (* environments are total *)
+Require Import densem.envSet. (* def of ENV , hide, constraints *)
+Require Import densem.densem. (* semantic definitions *)
+
+Import mini.MiniNotation.
+Import SetNotations.
+Import SetMonadNotation.
+Import List.ListNotations.
+Import ListMonadNotation.
+Import EnvNotation.
+Import envSetNotation.
+
+Open Scope list_scope.
+Open Scope mini_expr_scope.
+Open Scope env_scope.
+Open Scope set_scope.
+
+Import DLS.
+
+(* other distinguished variable (not equal to r) *)
+Definition x := mini.Test.x.
+Definition y := mini.Test.y.
+
+
+(* This is a bit of a hack. For examples, we special case the variables
+   x,y, and y when simplifying environment lookups *)
+
+Ltac rewrite_env := 
+  repeat match goal with 
+    | [ |- context[ (?x |-> ?v , ?rho) ?x ] ] => 
+        rewrite extend_lookup_same
+    | [ |- context[ (x |-> ?v , ?rho) r ] ] => 
+        rewrite extend_lookup_diff;
+        [rewrite PeanoNat.Nat.eqb_neq;easy|]
+    | [ |- context[ (y |-> ?v , ?rho) r ] ] => 
+        rewrite extend_lookup_diff;
+        [rewrite PeanoNat.Nat.eqb_neq;easy|]
+    | [ |- context[ (r |-> ?v , ?rho) x ] ] => 
+        rewrite extend_lookup_diff;
+        [rewrite PeanoNat.Nat.eqb_neq;easy|]
+    | [ |- context[ (r |-> ?v , ?rho) y ] ] => 
+        rewrite extend_lookup_diff;
+        [rewrite PeanoNat.Nat.eqb_neq;easy|]
+    | [ |- context[ (y |-> ?v , ?rho) x ] ] => 
+        rewrite extend_lookup_diff;
+        [rewrite PeanoNat.Nat.eqb_neq;easy|]
+    | [ |- context[ (x |-> ?v , ?rho) y ] ] => 
+        rewrite extend_lookup_diff;
+        [rewrite PeanoNat.Nat.eqb_neq;easy|]
+  end.
+
+
+(* -------------------------------------------------------- *)
+(* ---- examples / theory about extract / squash_pick ----- *)
+
+Lemma squash_pick_singleton {A} (v : A) : 
+  squash_pick [ ⌈ v ⌉ ] = ⌈ [v] ⌉.  
+  cbn.
+  set_simpl.
+  unfold Cons. set_simpl.
+  done.
+Qed.
+
+Example squash_pickExample :
+  squash_pick [  ⌈ (Int 0) ⌉ ; ⌈ (Int 1) ⌉ ] = 
+    (⌈ [ Int 0 ; Int 1 ] ⌉).
+cbn. set_simpl.
+unfold Cons. set_simpl.
+done.
+Qed.
+
+Lemma squash_pick_two_example :
+  squash_pick [ ⌈ (Int 0) ⌉ ∪ ⌈ (Int 1) ⌉ ] = 
+               (⌈ [ Int 0 ] ⌉ ∪ ⌈ [ Int 1 ] ⌉).
+Proof.
+  cbn. unfold Cons,If3. set_simpl.
+Admitted.
+
+
+Lemma extract_one {v} : 
+  extract r (r ≈ ⟨ v ⟩) = ⌈ (v, Total_set) ⌉.
+Proof. 
+eapply set_extensionality. intro ρ.
+unfold extract. 
+set_simpl.
+split.
+- move=>h.
+  set_crunch.
+  set_simpl.
+  f_equal.
+- destruct ρ as [w Δ].
+  intro h. inv h.
+  exists (r |-> v).
+  set_simpl.
+  done.
+Qed. 
+
+Lemma extract_example {k} :
+  extract r (x ≈ ⟨ k ⟩ ∩ r ≈ ⟨ k ⟩) = 
+    ⌈ (k, x ≈ ⟨ k ⟩) ⌉.
+Proof.
+  unfold extract.
+  eapply set_extensionality. intros [v Δ].
+  set_simpl.
+  split.
+  + intros h.
+    inv h.
+    set_crunch.
+    inv H.
+    repeat rewrite H2.  clear H2.
+    f_equal.
+    set_simpl.
+    rewrite constrain_eq_hide_two. done. done.
+  + intro h. inv h.
+    exists (x |-> k, r |-> k).
+    set_simpl.
+    rewrite_env.
+    rewrite constrain_eq_hide_two. done. done.
+Qed. 
+
+Lemma extract_two :
+  extract r (r ≈ ⟨ Int 0 ⟩ ∪ (r ≈ ⟨ Int 1 ⟩)) = 
+    (⌈ (Int 0, Total_set) ⌉ ∪ ⌈ (Int 1, Total_set) ⌉).
+Admitted.
+
+
+Lemma bcp_example : 
+  ALL [x ≈ ⟨ Int 0 ⟩ ∩ r ≈ ⟨ Int 0 ⟩] = 
+      ((x ≈ ⟨ Int 0 ⟩ ∩ r ≈ ⟨mkTup [Int 0]⟩) ∪
+       (x ≉ ⟨ Int 0 ⟩ ∩ r ≈ ⟨mkTup []⟩)).
+Proof.
+  unfold ALL.
+  apply set_extensionality. intros ρ.
+  unfoldIn.
+  unfold consistent_results.
+  list_simpl.
+  rewrite extract_example.
+  set_simpl.
+  unfold squash_pick.
+  remember (when (ρ ∈ x ≈ ⟨ Int 0 ⟩) ⌈ Int 0 ⌉) as ϕ.
+  split.
+  + intro h. 
+    crunch.
+    unfold If3 in H.
+    inv H. 
+    ++ set_crunch.
+       unfold Cons in H1.
+       set_crunch.
+       inv H2.
+       rewrite H3.
+       left. split; eauto.
+    ++ unfold when, guard in H1.
+       set_crunch.       
+       admit.
+Admitted.
+(*
+rewrite H1.
+       left.
+       have hh: (Int 0 = Int 0) = True. { apply propositional_extensionality. tauto. }
+       rewrite hh.
+       set_simpl.
+       reflexivity.
+    ++ exists nil.
+       cbn. 
+       set_crunch.
+       unfold constrain_ne,In in H0.
+       have hh: ((x ≈ ⟨ Int 0 ⟩) ρ) = False.
+       { unfold constrain_eq. 
+         eapply propositional_extensionality. tauto. }
+       rewrite hh. 
+       set_simpl.
+       eapply in_singleton.
+       auto.
+Qed. *)
+
+(* one { 0 | 1 } = [ {{ r = 0 }} ]     *)
+(* one { x = 0 } = [ {{ r = x = 0 }} ] *)
+(* one { x = 0 | x = 1 } = [ {{ r=x=0 }} union {{r=x=1}} ] *)
+
+Definition D0 : ENV := r ≈ ⟨ Int 0 ⟩.
+Definition D1 : ENV := r ≈ ⟨ Int 1 ⟩.
+Definition Dx v : ENV := x ≈ ⟨ v ⟩ ∩ r ≈ ⟨ v ⟩.
+
+
+Lemma extract_D0 : 
+  extract r D0 = ⌈ ( Int 0, Total_set ) ⌉. 
+Admitted.
+Lemma extract_D1 :
+  extract r D1 = ⌈ (Int 1 , Total_set) ⌉.
+Admitted.
+
+Lemma ONE_example1 : ONE [ D0 ; D1 ] = D0.
+Proof.
+  unfold ONE.
+  apply set_extensionality. intros ρ.
+  unfold consistent_results.
+  unfoldIn.
+  unfold List.map.
+  rewrite extract_D0. rewrite extract_D1.
+  set_simpl.
+  unfold squash_pick.
+  unfold Head.
+  split.
+  + intros h.
+    inv h.
+    inv H.
+Admitted.
+(*    inv H0. 
+    unfold D0, constrain_eq. 
+    autorewrite with set_simpl in H1. inv H1.
+  + unfold D0. 
+    intro h. inv h.
+    exists [ Int 0 ; Int 1].
+    rewrite H0.
+    split.
+    cbn.
+    set_simpl.
+    eapply in_singleton. cbn.
+    eapply in_singleton.
+Qed.
+*)
+
+Lemma ONE_example2 : 
+  ONE [ Dx (Int 0) ] = Dx (Int 0).
+Admitted.
+
+Lemma bind_when {A B} ϕ (s : P A) (k : A -> P B) : 
+  (bind (when ϕ s) k) = (⟨ϕ⟩ ∩ (bind s k)).
+Proof.
+Admitted.
+
+Lemma If3_when_ret {A B} (k : A) ϕ (s2 s3 : P B): 
+  If3 (when ϕ ⌈k⌉) s2 s3 = ((⟨ϕ⟩ ∩ s2) ∪ (⟨not ϕ⟩ ∩ s3)).
+Admitted.
+
+Lemma ONE_example3 : 
+  ONE [ Dx (Int 0) ; Dx (Int 1) ] = (Dx (Int 0) ∪ Dx (Int 1)).
+Proof.
+  unfold ONE, Dx, consistent_results.
+  apply set_extensionality. intros ρ.
+  unfoldIn.
+  unfold List.map.
+  repeat rewrite extract_example.
+  set_simpl.
+  split.
+  + intros h.
+    unfold Head, squash_pick in h.
+Admitted.    
+
+
+Lemma ALL_two_example :
+  ALL [(r ≈ ⟨Int 0⟩ ∪ (r ≈ ⟨Int 1⟩)) ] = 
+      (r ≈ ⟨mkTup [Int 0]⟩ ∪ (r ≈ ⟨mkTup [Int 1]⟩)).
+  apply set_extensionality. intros ρ.
+  set_simpl.
+  unfold ALL.
+  unfoldIn.
+  list_simpl. unfold consistent_results.
+  rewrite extract_two.
+  set_simpl.
+  repeat rewrite when_is_true; try easy.
+  rewrite squash_pick_two_example.
+  split.
+  + intro h. crunch.
+    inv H; inv H1. left; auto. right; auto.
+  + intro h. inv h.
+    exists [Int 0]. split; auto. left. eauto with sets.
+    exists [Int 1]. split; auto. right. eapply in_singleton. 
+Qed.
+
+Lemma conflict_example : 
+  ALL [ x ≈ ⟨ Int 0 ⟩ ∩ r ≈ ⟨ Int 0 ⟩ ; 
+         x ≈ ⟨ Int 1 ⟩ ∩ r ≈ ⟨ Int 1 ⟩ ]
+   = (((x ≈ ⟨ Int 0 ⟩) ∩ (r ≈ ⟨ mkTup [Int 0] ⟩))
+   ∪ ((x ≈ ⟨ Int 1 ⟩) ∩ (r ≈ ⟨ mkTup [Int 1] ⟩))
+   ∪ ((x ≉ ⟨ Int 0 ⟩) ∩ x ≉ ⟨ Int 1 ⟩ ∩ (r ≈ ⟨ mkTup []⟩))).
+Admitted.  
+
+
+Lemma squash_irr_ALL (s : list ENV) : 
+  ALL s = ALL (squash s).
+Proof.
+  unfold ALL.
+  eapply set_extensionality. intros ρ.
+  repeat unfoldIn.
+  split.
+  + intro h. crunch.
+    exists x0. split; auto.
+Abort.
+
+(* ---------------------------------------------------------- *)
+
+(*** IF examples and variants ***)    
+
+
+Definition negative_IF := 
+  mini.If3 (x :=: 0 :|: x :=: 1) (x :=: 1) mini.Fail.
+
+Notation "r ≈ x ≈ ⟨ k ⟩" := ((r ≈ ⟨ k ⟩) ∩ (x ≈ ⟨ k ⟩)) : set_scope.
+
+Lemma E_scrut :
+  E (x :=: 0 :|: x :=: 1) = [ (r ≈ x ≈ ⟨Int 0⟩) ; (r ≈ x ≈ ⟨Int 1⟩) ].
+Proof.
+  cbn. 
+Abort.  
+
+Lemma xNr x r (EQ: x <> r) : ~ Scope.In x ⟅ r ⟆.
+Admitted.
+
+Lemma rIr r : Scope.In r ⟅ r ⟆.
+Admitted.
+
+Lemma hidden_constrain x r k (NEQ: x <> r) :
+  (x ≈ ⟨ k ⟩) \ ⟅ r ⟆ = (x ≈ ⟨ k ⟩).
+unfold hidden. rewrite hide_constrain. eapply xNr. done. done.
+Qed.
+
+Hint Resolve hidden_constrain : sets.
+
+Lemma hide_result k:
+  (r ≈ x ≈ ⟨ k ⟩ \ ⟅ r ⟆) = x ≈ ⟨ k ⟩.
+Proof.
+  rewrite hide_intersection_r. eapply hidden_constrain; auto.
+  set_simpl. done.
+Qed.
+
+Lemma hide_arg k:
+  (r ≈ x ≈ ⟨ k ⟩ \ ⟅ x ⟆) = r ≈ ⟨ k ⟩.
+Proof.
+  rewrite hide_intersection_l. eapply hidden_constrain; auto.
+  set_simpl. done.
+Qed.
+
+
+Hint Rewrite hide_result hide_arg : sets.
+(*
+Lemma hide_example k: 
+  ((r ≈ x ≈ ⟨ k ⟩) ∩ r ≈ ⟨ k ⟩ \ ⟅ r ⟆) = x ≈ ⟨ k ⟩.
+Admitted.
+*)
+Lemma constrain_same1 r x k : 
+  (r ≈ x ≈ ⟨ k ⟩ ∩ r ≈ ⟨ k ⟩) = (r ≈ x ≈ ⟨ k ⟩).
+Admitted.
+
+Lemma constrain_same2 r x k : 
+  (r ≈ ⟨ k ⟩ ∩ (r ≈ x ≈ ⟨ k ⟩)) = (r ≈ x ≈ ⟨ k ⟩).
+Admitted.
+
+Lemma constrain_same3 r x k : 
+  (x ≈ ⟨ k ⟩ ∩ (r ≈ x ≈ ⟨ k ⟩)) = (r ≈ x ≈ ⟨ k ⟩).
+Admitted.
+
+Lemma constrain_same4 r x k : 
+  (r ≈ x ≈ ⟨ k ⟩ ∩ x ≈ ⟨ k ⟩) = (r ≈ x ≈ ⟨ k ⟩).
+Admitted.
+
+
+Hint Rewrite constrain_same1 constrain_same2 constrain_same3 constrain_same4 : sets.
+
+Lemma constrain_conflict0 k1 k2 (NE : k1 <> k2) :
+  (x ≈ ⟨ k1 ⟩) ∩ (x ≈ ⟨ k2 ⟩) = ∅.
+Admitted.
+
+Lemma constrain_conflict1 k1 k2 (NE : k1 <> k2) :
+  (x ≈ ⟨ k1 ⟩) ∩ (r ≈ x ≈ ⟨ k2 ⟩) = ∅.
+Admitted.
+
+Lemma constrain_conflict2 k1 k2 (NE : k1 <> k2) :
+ (r ≈ ⟨ k1 ⟩) ∩ (x ≈ ⟨ k1 ⟩) ∩ ((x ≈ ⟨ k2 ⟩ ∪ x ≈ ⟨k1⟩)) = (r ≈ ⟨ k1 ⟩) ∩ (x ≈ ⟨ k1 ⟩).
+Admitted.
+
+Lemma Setminus_disjoint1 k1 k2 (NEQ: k1 <> k2) :
+  (x ≈ ⟨ k1 ⟩) - (x ≈ ⟨ k2 ⟩) = (x ≈ ⟨ k1 ⟩).
+Admitted.
+
+Lemma Setminus_disjoint k1 k2 (NEQ: k1 <> k2) :
+  (r ≈ x ≈ ⟨ k1 ⟩) - (r ≈ ⟨ k2 ⟩) = (r ≈ x ≈ ⟨ k1 ⟩).
+Proof.
+  unfold Setminus.
+  set_ext ρ. unfoldIn.
+  split. 
+  + intros [h1 h2].
+    set_crunch.
+    split. unfold constrain_eq. unfoldIn. auto.
+    unfold constrain_eq. unfoldIn. auto.
+  + intros [h1 h2].
+    set_crunch; unfold constrain_eq; try split; try unfoldIn; auto.
+    congruence.
+Qed.
+
+(* if (x: = (0 |1)) { x = 1 } else {fail} == [ 1 ] *)
+(* Tim wants this to fail. *)
+Lemma IF_Tim_choice : 
+  IF_TIM ⟅x⟆ ([ (r ≈ x ≈ ⟨Int 0⟩) ; (r ≈ x ≈ ⟨Int 1⟩) ]) [(r ≈ x ≈ ⟨Int 1⟩) ] [] = 
+  [∅; r ≈ ⟨ Int 1 ⟩].
+unfold IF_TIM.
+cbn.
+set_simpl.
+repeat rewrite hide_result; auto.
+rewrite constrain_conflict1; try done.
+rewrite Setminus_disjoint1; try done.
+set_simpl.
+rewrite constrain_same3.
+rewrite hide_arg; auto.
+Qed.
+
+
+Lemma IF_Tim_choice_no_bind : 
+  IF_TIM (Scope.empty) 
+    ([ (r ≈ x ≈ ⟨Int 0⟩) ; (r ≈ x ≈ ⟨Int 1⟩) ]) 
+         [(r ≈ x ≈ ⟨Int 1⟩) ] [] = 
+  [∅; r ≈ x ≈ ⟨ Int 1 ⟩].
+unfold IF_TIM.
+cbn.
+set_simpl.
+repeat rewrite hide_result; auto.
+rewrite constrain_conflict1; try done.
+rewrite Setminus_disjoint1; try done.
+rewrite constrain_same3.
+auto.
+Qed.
+
+
+Lemma IF_Tim_choice_ifxx : 
+  IF_TIM (Scope.empty) 
+    ([ (r ≈ x ≈ ⟨Int 0⟩) ; (r ≈ x ≈ ⟨Int 1⟩) ]) 
+         [(r ≈ ⟪x⟫) ] [] = 
+  [r ≈ x ≈ ⟨Int 0⟩; r ≈ x ≈ ⟨ Int 1 ⟩].
+Proof.
+unfold IF_TIM.
+cbn.
+set_simpl.
+repeat rewrite hide_result; auto.
+f_equal. admit.
+rewrite Setminus_disjoint1; try done.
+f_equal.
+admit.
+Admitted.
+
+
+Lemma IF_Tim_choice_ifxxscoped : 
+  IF_TIM ⟅x⟆ 
+    ([ (r ≈ x ≈ ⟨Int 0⟩) ; (r ≈ x ≈ ⟨Int 1⟩) ]) 
+         [(r ≈ ⟪x⟫) ] [] = 
+  [r ≈ ⟨Int 0⟩; r ≈ ⟨ Int 1 ⟩].
+Proof.
+unfold IF_TIM.
+cbn.
+set_simpl.
+repeat rewrite hide_result; auto.
+f_equal. admit.
+rewrite Setminus_disjoint1; try done.
+f_equal.
+admit.
+Admitted.
+
+
+
+(* if (x: = 0 | x = 1) { x = 1 } else {fail} == [ 1 ] *)
+Lemma IF_SPJ_choice : 
+  IF_SPJ ⟅x⟆ ([ (r ≈ x ≈ ⟨Int 0⟩) ; (r ≈ x ≈ ⟨Int 1⟩) ]) [(r ≈ x ≈ ⟨Int 1⟩) ] [] = 
+  [r ≈ ⟨ Int 1 ⟩].
+unfold IF_SPJ.
+cbn.
+set_simpl.
+repeat rewrite hide_result; auto.
+rewrite constrain_conflict2; try done.
+rewrite hide_arg.
+auto.
+Qed.
+
+(* if (x = 0 | x = 1) { x = 1 } else {fail} == [ x = 1 ] *)
+Lemma IF_SPJ_choice_no_bind : 
+  IF_SPJ (Scope.empty) ([ (r ≈ x ≈ ⟨Int 0⟩) ; (r ≈ x ≈ ⟨Int 1⟩) ])
+     [(r ≈ x ≈ ⟨Int 1⟩) ] [] = 
+  [r ≈ x ≈ ⟨ Int 1 ⟩].
+Proof.
+unfold IF_SPJ.
+cbn.
+set_simpl.
+repeat rewrite hide_result; auto.
+rewrite constrain_conflict2; try done.
+Qed.
+
+
+Lemma extract_xisk k : 
+  extract r (r ≈ x ≈ ⟨k⟩) = ⌈ (k, x ≈ ⟨k⟩) ⌉.
+unfold extract. set_simpl.
+unfold Sets.map.
+set_ext ρ. unfoldIn.
+split.
+- intro h. set_crunch. eapply in_singleton'.
+  f_equal. set_simpl. 
+  admit.
+- intro h. set_crunch.
+  exists (x |-> k, r|-> k). split. 
+  f_equal.
+  rewrite_env. 
+  admit.
+Admitted.
+
+Hint Unfold constrain_eq : sets.
+
+(*
+Lemma ONEchoice :
+  ONE [ (r ≈ x ≈ ⟨Int 0⟩) ; (r ≈ x ≈ ⟨Int 1⟩) ] = ∅.
+Proof.
+  unfold ONE.
+  unfold List.map.
+  unfold consistent_results.
+  repeat rewrite extract_xisk.
+  set_ext ρ.
+  split.
++ intro h. inv h.
+  set_simpl in H.
+*)
+
+Lemma ONEresolved_example :
+  (r ≈ x ≈ ⟨Int 1⟩) ∩ ONE [ (r ≈ x ≈ ⟨Int 0⟩) ; (r ≈ x ≈ ⟨Int 1⟩) ] =
+    (r ≈ x ≈ ⟨Int 1⟩).
+Proof.  
+  unfold ONE.
+  unfold List.map.
+  unfold consistent_results.
+  repeat rewrite extract_xisk.
+  set_simpl.
+  set_ext ρ.
+  split. 
++ 
+  intros h.
+  set_crunch.
+  set_simpl in H0.
+  destruct x0. done.
+  inv H2.
+  unfold squash_pick in H0.
+  rewrite when_is_false in H0. intro h. inv h. rewrite H4 in H0. inv H0.
+  set_simpl in H0. rewrite H4.
+  rewrite when_is_true in H0. auto with sets. 
+  auto with sets. 
++ intro h. set_crunch. rewrite H2.
+  split. auto with sets. split. auto with sets.
+  unfoldIn.
+  set_simpl.
+  rewrite when_is_false. intro h. inv h. rewrite H2 in H0. done.
+  rewrite when_is_true. auto with sets.
+  unfold squash_pick. set_simpl.
+  unfold Cons, Head. set_simpl.
+  done.
+Qed.
+
+(**** SIMON's derivation of IF encoded using one. *)
+
+(* Ed[ e1; r=<> ] = [ hide(r) D1 ∩ {{ r=<> }} | D1 <- E[e1] ] *)
+Lemma part1 e1 : E (e1 :>: r :=: mini.Array []) = 
+        List.map (fun D1 => hide ⟅r⟆ D1 ∩ (r ≈ ⟨mkTup []⟩)) (E e1).
+Proof.
+  cbn.
+  unfold UNIFY.
+  unfold hide_list.
+  set_simpl.
+Admitted.
+
+(*
+Ed[ (e1; r=<>) | r=0 ] = [ hide_r D1 \cap {{r=<>}} | D1 <- E[e1] ] ++ [ {{r=0}} ] 
+*)
+Lemma part2 e1 : E ( (e1 :>: r :=: mini.Array []) :|: r :=: 0) = 
+                List.map (fun D1 => hide ⟅r⟆ D1 ∩ (r ≈ ⟨mkTup []⟩)) (E e1) ++ [ r ≈ ⟨Int 0⟩ ].
+rewrite E_Choice. 
+rewrite part1.
+cbn. set_simpl. done.
+Qed.
+
+(* ---- y = one{ (e1; z=<>) | z=0}@z -------------
+  Ed[ y = one{(e1; z=<>) | z=0}@z ]
+
+= [ { rho | v =<>,  
+      if rho ∈ UNIONLIST (map hide(z) E[e1])   # UNIONLIST :: [ENV] -> ENV, union them all
+               = 0,   otherwise
+     , rho y = v } ]
+*)
+
+
+Definition if2 (ϕ1 : Prop) (ϕ3 : Prop) := 
+  (~ ϕ1 /\ ϕ3).
+
+Definition if3 (ϕ1 : Prop) (ϕ2 : Prop) (ϕ3 : Prop) := 
+  (ϕ1 /\ ϕ2) \/ (~ ϕ1 /\ ϕ3).
+
+Lemma if3_rhoIn (S1 S2 S3 : ENV) :
+  [ (fun ρ => if3 (ρ ∈ S1) (ρ ∈ S2) (ρ ∈ S3)) ] = 
+  [(S1 ∩ S2) ∪ (Total_set - S1 ∩ S3)].
+Proof.
+  unfold if3.
+  replace (fun ρ : env => ρ ∈ S1 /\ ρ ∈ S2 \/ ~ ρ ∈ S1 /\ ρ ∈ S3) with 
+          ((fun ρ => ρ ∈ S1 /\ ρ ∈ S2) ∪ (fun ρ => ~ ρ ∈ S1 /\ ρ ∈ S3)).
+  2: { set_ext ρ. rewrite in_union. intuition. }
+  replace (fun ρ => ρ ∈ S1 /\ ρ ∈ S2) with (S1 ∩ S2).
+  2: { set_ext ρ. rewrite in_intersection. intuition. inv H. auto. inv H. auto. } 
+  replace (fun ρ => ~ ρ ∈ S1 /\ ρ ∈ S3) with (Total_set - S1 ∩ S3).
+  2: { set_ext ρ. rewrite in_intersection. unfoldIn.
+       intuition. inv H0. done. unfold Total_set, Setminus. unfoldIn. intuition. }
+  done.
+Qed.
+
+Lemma squash_pick_app : 
+  forall {A} (xs ys : list (P A)), squash_pick (xs ++ ys) = 
+             xs' ⭅ (squash_pick xs) ;; 
+             ys' ⭅ (squash_pick ys) ;; 
+             ⌈ xs' ++ ys' ⌉ .
+Proof. 
+  induction xs.
+  + intros ys. cbn. 
+    set_simpl.
+    reflexivity.
+  + intros ys.
+    cbn.
+    have h: ((Inhabited a) \/ (a = ∅)). admit.
+    inv h.
+    ++ repeat rewrite If3_nonempty; auto.
+       rewrite IHxs.
+       unfold Cons.
+       set_simpl.
+       f_equal.
+       apply functional_extensionality. intro v.
+       set_simpl.
+       f_equal.
+       apply functional_extensionality. intro vs.
+       rewrite Sets.bind_bind.
+       rewrite Sets.bind_singleton_l.
+       f_equal.
+       apply functional_extensionality. intro ws.
+       set_simpl.
+       done.
+    ++ repeat rewrite If3_empty; auto.
+Admitted.
+
+
+(* = 
+   Ed[ y = one{(e1; z=<>) | z=0}@z ]
+   = [ { rho | v  = tup[],  if rho ∈ UNIONLIST (map hide(z) E[e1]) 
+                  = 0,      otherwise
+             , rho y = v } ]
+*)
+
+Lemma if3_union: forall (S1 S1' : Prop) (S2 S3 : Prop),  
+                if3 (S1 \/ S1') S2 S3 = if3 S1 S2 (if3 S1' S2 S3).
+Proof.
+ intros. unfold if3. 
+ apply propositional_extensionality. tauto. Qed.
+
+Lemma part3 e1 : 
+    E (y :=: mini.One ((e1 :>: r :=: mini.Array []) :|: r :=: 0)) = 
+      let GOOD := UNIONLIST (List.map hide_r (E e1)) in
+      [ (GOOD ∩ (r ≈ y ≈ ⟨mkTup []⟩)) 
+      ∪ ((Total_set - GOOD) ∩ (r ≈ y ≈ ⟨Int 0⟩)) ].
+Proof.
+  rewrite E_Unify.
+  rewrite E_One.
+  rewrite part2.
+  rewrite hide_nothing.
+  rewrite E_Var.
+  unfold UNIFY.
+  list_simpl.
+
+  remember (fmap (fun D2 : ENV => hide_r D2 ∩ r ≈ ⟨ mkTup [] ⟩) (E e1) ++ [r ≈ ⟨ Int 0 ⟩]) as Δs.
+
+  rewrite <- if3_rhoIn.
+  remember (UNIONLIST (List.map hide_r (E e1))) as GOOD.
+
+  unfold ONE.
+
+  f_equal.
+  set_ext ρ. rewrite in_intersection. 
+
+  unfold In. 
+  remember  (List.map (consistent_results ρ) Δs) as S.
+  rewrite HeqΔs in HeqS.
+  unfold fmap, Functor_list in HeqS.
+  rewrite List.map_app in HeqS.
+  rewrite List.map_map in HeqS.
+  rewrite list_map_singleton in HeqS.
+  unfold consistent_results in HeqS.
+  rewrite extract_one in HeqS.
+  set_simpl in HeqS.
+  rewrite when_is_true in HeqS; [unfold Total_set;done|].
+
+  replace (fun x : ENV => x0 ⭅ extract (hide_r x ∩ r ≈ ⟨ mkTup [] ⟩);; 
+                       (let (v, Δ') := x0 in when (ρ ∈ Δ') (⌈v⌉)))
+     with (fun x : ENV => when (ρ ∈ hide_r x) (⌈mkTup []⌉)) 
+  in HeqS.
+  2: { 
+    apply functional_extensionality. intro Δ1.
+    unfold extract.
+    admit.
+  } 
+  subst.
+  rewrite squash_pick_app.
+
+  cbn.
+  rewrite If3_nonempty. econstructor;econstructor; eauto.
+  unfold Cons. set_simpl.
+  
+  split.
+  + intros h. crunch. 
+    rewrite H in H0. 
+    unfold Head in H0. 
+    set_simpl in H0.
+    inv H0; crunch.
+    inv H1; crunch.
+    set_simpl in H1.
+    destruct x0. 
+    ++ (* squash_pick fails *) 
+      inv H1.
+      cbn in H2. inv H2.
+
+       right. split; auto. 
+       2: { unfold constrain_eq. split. unfoldIn. done.
+            unfoldIn. done. }
+       intro h.
+
+       remember (E e1) as VS.
+       move: H0 h.
+       clear.
+       (* need to prove that it fails *)
+       move: ρ.
+       induction VS; intro ρ.
+       - cbn. done.
+       - intros. 
+         replace (a :: VS) with ([a] ++ VS) in H0. 2: { auto. } 
+         rewrite List.map_app in H0.
+         rewrite squash_pick_app in H0.
+         inv H0; crunch.
+         rewrite List.map_singleton in H.
+         cbn in H.
+         inv H0; crunch.
+         destruct x0. 2: { inv H1. } 
+         destruct x1. 2: { inv H1. } 
+         cbn in h. inv h.
+         -- rewrite when_is_true in H; auto.
+            rewrite If3_nonempty in H. econstructor; econstructor; eauto.
+            unfold Cons in H.
+            autorewrite with set_simpl in H.
+            inv H.
+         -- apply IHVS in H0. done. auto.
+    ++ (* squash pick succeeds *)
+      inv H1. clear H3.
+      remember (E e1) as VS.
+      clear HeqVS.
+      cbn in H2. inv H2.
+      induction VS as [|W WS].
+      - inv H0.
+      - cbn.
+        cbn in H0.
+        have CL: (ρ ∈ hide_r W) \/ ~(ρ ∈ hide_r W). admit.
+        destruct CL.
+        -- (* first one works *) 
+          clear IHWS.
+          rewrite when_is_true in H0; auto.
+          rewrite If3_nonempty in H0. econstructor; econstructor; eauto.
+          unfold Cons in H0.
+          set_simpl in H0.
+          inv H0; crunch.
+          inv H0; crunch.
+          clear H2.
+
+          replace ((hide_r W ∪ UNIONLIST (ListDef.map hide_r WS)) ρ) with
+            ((ρ ∈ hide_r W) \/ (ρ ∈ UNIONLIST (ListDef.map hide_r WS))). 2: { unfold In. admit. } 
+                                                                      
+          rewrite if3_union.
+          unfold if3. left. split. auto. split; eauto. 
+          rewrite H4. unfold constrain_eq. unfold In. done.
+      -- (* first one doesn't *)
+        rewrite when_is_false in H0; auto.
+        autorewrite with set_simpl in H0.
+        move: (IHWS H0) => ih. clear IHWS H0.
+        replace ((hide_r W ∪ UNIONLIST (ListDef.map hide_r WS)) ρ) with
+            ((ρ ∈ hide_r W) \/ (ρ ∈ UNIONLIST (ListDef.map hide_r WS))). 2: { admit. } 
+        rewrite if3_union.
+        unfold if3.
+        right.
+        split. auto.
+        unfold if3 in ih.
+        inv ih; crunch. left. split. auto. auto.
+        right. split. auto. auto.
+ + intro h.
+   unfold if3 in h.
+   destruct h.
+   ++ (* ρ in UNIONLIST (E e1 \ r) *)
+     crunch.
+     inv H0. inv H1. done.
+     inv H0. inv H1. inv H2.
+     unfold Head.
+     set_simpl.
+Admitted.
+
+(* y = one{ (e1; z=<>) | z=0}@z; (y=⟨⟩; e2) | (y=0; e3)  
+  [ GOOD ⋂ {{y=<>}} ⋂ D | D ∈ Ed[e2] ] ++
+  [ BAD ⋂ {{y=0}}   ⋂ D  | D ∈ Ed[e3] ]
+*)
+
+Lemma UNIONLIST_hide VS s :
+  UNIONLIST (VS [\] s) = ((UNIONLIST VS) \ s).
+induction VS.
+cbn. set_simpl. done.
+cbn. set_simpl. f_equal.
+auto.
+Qed.
+
+Lemma part4 e1 e2 e3 : 
+  E (y :=: mini.One (e1 :>: r :=: mini.Array [] :|: r :=: 0) 
+       :>: 
+    ((y :=: mini.Array [] :>: e2) :|: (y :=: 0 :>: e3))) = 
+  let GOOD := UNIONLIST (List.map hide_r (E e1)) in
+  let BAD  := Total_set - GOOD in 
+  (List.map (fun D => GOOD ∩ (y ≈ ⟨mkTup []⟩) ∩ D) (E e2)) ++
+  (List.map (fun D => BAD  ∩ (y ≈ ⟨Int 0⟩) ∩ D) (E e3)).
+Proof.
+  rewrite E_Seq.
+  rewrite part3.
+  rewrite E_Choice.
+  repeat rewrite E_Seq.
+  repeat rewrite E_Unify.
+  repeat rewrite E_Var.
+  cbn.
+  remember (UNIONLIST (ListDef.map hide_r (E e1))) as GOOD.
+  remember (Total_set - GOOD) as BAD.
+  repeat rewrite flat_map_map.
+  repeat rewrite List.app_nil_r.
+  repeat rewrite List.map_app.
+  repeat rewrite List.map_map.
+  f_equal.
+  - f_equal.
+    apply functional_extensionality. intro D.
+    set_simpl.
+    set_ext ρ.
+    split.
+    ++ set_simpl.
+       intros [h1 h2].
+       inv h2. inv H. inv H1. inv H. inv H3. inv H1.
+       have NI: ~ Scope.In y ⟅ r ⟆. { admit. }
+       move: (H2 y ltac:(eauto))=> NY.
+       repeat split; try congruence.
+       inv h1.
+       -- unfold hide in H. inv H. 
+          inv H1.
+          inv H.
+          unfold constrain_eq in H6. inv H6. inv H. inv H7.
+          rewrite UNIONLIST_hide in H1. inv H1. crunch.
+          rewrite UNIONLIST_hide. unfold hide.
+          exists x2. split; auto. intros z zIn. rewrite H5; auto.
+       -- unfold hide in H. inv H. crunch.
+          inv H. unfold constrain_eq in H6.
+          inv H6. inv H. inv H7.
+          rewrite <- H1 in H6; auto.
+          rewrite H2 in H6; auto.
+          rewrite <- H3 in H6.
+          rewrite H4 in H6.
+          inv H6.
+    ++ set_simpl. 
+       intro h. inv h. inv H0.
+       split.
+       left.
+       rewrite  UNIONLIST_hide.
+       unfold hide. unfoldIn.
+       rewrite UNIONLIST_hide in H.
+       unfold hide in H. destruct H as [ρ' H].
+       inv H.
+       exists (r |-> mkTup [], ρ). repeat split.
+Admitted.
+
+
+(* E [if (x=1|x=2) { x } { 0 }] = [ {r=1,x=1} | {r=2,x=2} | {r=0,x<>1,2} *)
+Definition if_iter := mini.If3 (x :=: 1 :|: x :=: 2) x 0.
+
+(** other examples **)
+
+
+(* if(a){b}else{c} <=> if(a){b}else{:false} | if(a){:false}else{c} *)
+Lemma opinionated_if a b c: 
+  E(mini.If3 a b c) =  E( mini.If3 a b mini.Fail :|: mini.If3 a mini.Fail c).
+Proof. 
+  unfold E. fold E.
+  destruct (try (mini.I a) (E a)) as [success avoid].
+  replace (SEQ [Total_set - avoid] []) with ([] : list ENV).
+  2 : { cbn. auto. } 
+  rewrite -> List.app_nil_r.
+  replace (SEQ success ([] [\] mini.I a)) with ([] : list ENV).
+  2: { cbn. unfold SEQ, UNIFY. cbn.
+       admit. } 
+  rewrite -> List.app_nil_l. auto.
+Admitted.
+
+
+
+(* 
+
+if e1 e2 e3 =
+  exists y; 
+  y = one{ (e1; z=⟨⟩) | z=0 }@z;
+  (y=⟨⟩; e2) | (y=0; e3)
+
+koen_if =
+  fun e1 e2 e3 : mini.Expr =>
+  ∃ y :>: 
+  y :=: mini.One (e1 :>: r :=: mini.Array [] :|: r :=: 0) :>: 
+  y :=: mini.Array [] :>: e2 :|: y :=: 0 :>: e3
+*)
+
+(*
+= [ D ⋂ GOOD | D ∈ Ed[e2] ] ++
+  [ D \ GOOD | D ∈ Ed[e3] ]
+where
+  GOOD :: ENV = UNIONLIST (map hide(r) Ed[e1])
+
+*)
+
+End D_LS_Theory.
