VerseRocq/verse/densem/examplesELV.v
@@ -1,0 +1,388 @@
+Require Import Imports.
+
+From Stdlib Require Lists.List.
+From Stdlib Require Import Classes.EquivDec.
+Import ssreflect.
+
+From Stdlib Require Import Logic.PropExtensionality.
+From Stdlib Require Import Logic.FunctionalExtensionality.
+From Stdlib Require Import Sets.Classical_sets.
+
+Require Import syntax.common.
+Require syntax.mini.
+Require Import PFun.
+Require Import structures.Sets.
+Import structures.List.
+
+Require Import densem.Dom.
+Require Import densem.tenv.  (* environments are total *)
+Require Import densem.envSet. (* def of ENV , hide, constraints *)
+Require Import densem.squash.
+
+Import mini.MiniNotation.
+Import SetNotations.
+Import SetMonadNotation.
+Import List.ListNotations.
+Import ListMonadNotation.
+Import EnvNotation.
+Import envSetNotation.
+
+Open Scope list_scope.
+Open Scope mini_expr_scope.
+Open Scope env_scope.
+Open Scope set_scope.
+
+Import ELV.
+
+(* ----------------------- examples --------------- *)
+
+Definition eval_top t d := eval Env.empty t d.
+
+
+Ltac ego := eauto with sets ; 
+            cbn ; 
+            try rewrite Intersection_same ;
+            try (rewrite Intersection_diff ; 
+                 [ intros ? ; discriminate| eauto with sets]) ;
+            eauto with sets.
+
+Ltac eeval1 := match goal with 
+              | [ |- eval ?env ?e ?VS ] =>
+                  econstructor ; eauto end.
+
+
+Ltac eeval := match goal with 
+              | [ |- eval ?env (mini.Seq _ _) ?VS ] =>
+                  econstructor ; 
+                  [ eeval | eauto with sets | eeval 
+                  | eauto with sets 
+                  | cbn ; eauto with sets ]
+              | [ |- eval ?env (mini.Unify _ _) ?VS ] =>
+                  econstructor ; [ eeval | eeval | ego ]
+              | [ |- eval ?env (mini.Var _) ?VS ] =>
+                  econstructor ; cbn ; eauto 
+              | [ |- eval ?env ?e ?VS ] =>
+                  econstructor ; eauto end.
+
+
+
+
+Lemma not_r : forall (x r : Ident), (SetoidList.InA eq x [r] -> False) -> Nat.eqb r x = false. Admitted.
+
+
+
+Lemma hide_constraint {i v} : (i ≈ fun _ => v) \ (Scope.singleton i) ≃ Total_set.
+split. 
+intros x xIn. cbv. auto.
+intros ρ ρIn. cbv.
+eexists.
+instantiate (1 := i |-> v, ρ).
+split. rewrite extend_lookup_same. auto.
+intros x NI. 
+apply not_r in NI. rewrite extend_lookup_diff; auto.
+Qed.
+
+Lemma hide_all s : (hide s Total_set) = Total_set.
+  eapply Extensionality_Ensembles.
+  split.
+  intros x xIn. cbv. auto.
+  intros x xIn. unfold hide.
+  exists x. split. auto.
+  intros y IH. auto.
+Qed.
+
+
+
+Lemma SEQ_SUCCEED_X X : SEQ SUCCEED X = X.
+  unfold SEQ, UNIFY, hide_list, SUCCEED.
+  cbn.
+  rewrite hide_all.
+  rewrite List.app_nil_r.
+  induction X.
+  - cbn. auto.
+  - cbn. f_equal.
+    eapply all_intersect.
+    auto.
+Qed.
+
+Example ex_ALL : 
+  (r |-> mkTup [Int 3;Int 4]) ∈ (ALL [ r ≈ ⟨3⟩;  r ≈ ⟨4⟩] ).
+cbn. exists ([Int 3; Int 4], Total_set).
+split; [exists (Int 3, Total_set);split|idtac]. 
+- cbv. extensionality ρ.
+  eapply propositional_extensionality.
+  split; try done. intro h.
+  exists (Env.extend r (Int 3) ρ). 
+  split. split. cbv. auto. cbv. auto.
+  intros x xIn. apply not_r in xIn. 
+  cbv. destruct x. done. done.
+- cbv.
+Admitted.
+
+
+Example first_example_none {A} : @first A  [ ∅ ] = ∅ .
+  eapply Extensionality_Ensembles. split.
+  - move => y yIn. 
+    unfold first in yIn. cbv in yIn.
+    inversion yIn; inversion H; subst; auto.
+  - move => y yIn. done.
+Qed.
+
+Example first_example {A} (x:A) : first  [ ∅ ; ∅ ; ⌈ x ⌉ ] = ⌈ x ⌉.
+Proof.
+  eapply Extensionality_Ensembles. split.
+  - move => y yIn. 
+    inversion yIn; inversion H; subst.
+    eapply not_Singleton_empty; eauto.
+    auto.
+  - move => y yIn.
+    right.
+    split. intro h. eapply not_Singleton_empty; eauto. auto.
+Qed.
+
+Example apply_tup0 x y : apply (mkTup [x;y]) (Int 0) = [ ⌈ x ⌉ ; ∅ ]. cbn. auto. Qed.
+Example apply_tup1 x y : apply (mkTup [x;y]) (Int 1) = [ ∅ ; ⌈ y ⌉ ]. cbn. auto. Qed.
+Example apply_add1 : apply Prim.add1 (Int 0) = [ ⌈ Int 1 ⌉ ]. cbn. auto. Qed.
+Example apply_isInt : apply Prim.isInt (Int 1) = [ ⌈ Int 1 ⌉ ]. cbn. auto. Qed.
+
+Example DODGY_UNIONS_ex : 
+  DODGY_UNIONS (⌈ [ ∅ ; ⌈ 3 ⌉ ] ⌉ ∪ ⌈ [ ⌈ 4 ⌉ ] ⌉) = 
+    [  ⌈ 4 ⌉ ; ⌈ 3 ⌉ ].
+Proof.
+  unfold DODGY_UNIONS, allNums. 
+  replace limitNum with 2.
+  cbn.
+  repeat rewrite map_union. repeat rewrite map_singleton.
+  cbn.
+  repeat rewrite -> UNION_union. 
+Admitted.  
+
+
+Module Test.
+
+Coercion Dom.Int : nat >-> value.
+
+(*   {y:=if(x=1){0|1}else{2|3}; x:=0|1; y}  =?= 2|0|3|1 *)
+
+Definition y := mini.Test.y.
+Definition x := mini.Test.x.
+
+Definition lennart := 
+  { y :=: mini.If3 (mini.Unify x 1) (0 :|: 1) (2 :|: 3) :>: 
+    x :=: (0 :|: 1)  :>:
+    y }.
+
+Lemma dodgy : eval Env.empty lennart 
+                ([ ⌈ Dom.Int 2 ⌉ ; ⌈ Dom.Int 0 ⌉ ; ⌈ Dom.Int 3 ⌉ ; ⌈ Dom.Int 1 ⌉ ]).
+Proof.
+  unfold lennart.
+  eeval.
+  instantiate (1 := 
+    (mem [ [ ⌈ Dom.Int 2 ⌉ ; ⌈ Dom.Int 0 ⌉ ; ⌈ Dom.Int 3 ⌉ ; ⌈ Dom.Int 1 ⌉ ] ;
+           [ ⌈ Dom.Int 2 ⌉ ; ⌈ Dom.Int 0 ⌉ ; ⌈ Dom.Int 3 ⌉ ; ⌈ Dom.Int 1 ⌉ ] ])).
+  intros WS WSIn.
+  apply mem_In in WSIn.
+  destruct WSIn.
+  - (* first option *)
+    exists ( (Env.extend y (Dom.Int 2) (Env.extend x (Dom.Int 1) Env.empty))).
+Admitted.
+
+
+Lemma t1 : eval_top mini.Test.t1 [ ⌈ Dom.Int 2 ⌉ ].
+Proof. unfold mini.Test.t1, eval_top. repeat eeval. Qed.
+
+
+(* { x:=1; x }  *)
+Lemma t2 : 
+  eval Env.empty mini.Test.t2 [ ⌈ Dom.Int 1 ⌉ ].
+Proof. unfold mini.Test.t2.
+       (* set up the block. *)
+       eeval1.
+       instantiate (1 := mem [ [ ⌈ Dom.Int 1 ⌉] ]).
+       intros WS WSIn.
+       2: { rewrite UNIONS_mem. cbn. eapply in_singleton. } 
+       apply mem_In in WSIn. cbn in WSIn.
+       destruct WSIn. 
+       - subst.
+         exists (mini.Test.x |-> Dom.Int 1 ).
+         split; auto.
+(*
+         ++ intros y.
+            destruct Scope.mem eqn:IN.
+            -- (* in new scope *) 
+              unfold mini.I in IN.
+              cbn in IN. fold Nat.compare in IN.
+              destruct Nat.compare eqn:CMP; try done.
+              apply PeanoNat.Nat.compare_eq in CMP. subst.
+              eexists. cbn. eauto. 
+            -- (* in old scope *)
+              unfold mini.I in IN.
+              cbn in IN. fold Nat.compare in IN.
+              destruct Nat.compare eqn:CMP; try done.
+              apply PeanoNat.Nat.compare_lt_iff in CMP.
+              admit.
+              admit.
+         ++ eeval.
+       - done. *)
+Admitted.
+
+
+
+(* No block here. *)
+(* x:=1; y:= if(x=2) then 0 else 3; y *)
+
+Lemma t7 : 
+  exists vx, exists vy, eval (Env.extend mini.Test.x vx (Env.extend mini.Test.y vy Env.empty)) mini.Test.t7 [ ⌈ Dom.Int 3 ⌉ ].
+Proof.  exists (Dom.Int 1). exists (Dom.Int 3).
+        unfold mini.Test.t7.
+        eapply eval_Seq.
+        - eeval.
+        - ego.
+        - eapply eval_Seq.
+          + eeval.
+          + ego.
+          + eapply eval_Seq.
+            -- eeval.
+            -- ego.
+            -- eapply eval_Unify.
+               ++ eeval.
+               ++ eeval1.
+                  +++ eapply eval_If3_false.
+                  --- intros rho' rho'X.
+                      unfold X, Ensembles.In in rho'X. 
+Admitted.
+(*
+                      move: (rho'X mini.Test.x) => [h _].
+                      cbn in h.
+                      specialize (h (Dom.Int 1) ltac:(auto)).                       
+                      eeval.
+                  --- eeval.
+               ++ ego.
+            -- ego.
+            -- ego.
+          + ego.
+          + ego.
+        - ego.
+        - ego.
+Qed.
+*)
+End Test.
+
+
+Module Theory.
+
+Lemma NonEmptyTail_UNIONS : 
+  forall V VV, 
+    UNIONS VV V -> 
+    (forall VS, VS ∈ VV -> NonEmptyTail VS) -> 
+    NonEmptyTail V.
+Proof.
+  intro V. induction V.
+  - intros.
+    unfold UNIONS in *.
+    unfold NonEmptyTail.
+    cbn. eauto with sets.
+  - intros VV VH U.    
+    unfold UNIONS in *.
+Admitted.
+
+Lemma NonEmptyTail_app {A} ( VS1 VS2 : list (P A)) : 
+  NonEmptyTail VS1 -> NonEmptyTail VS2 ->
+  NonEmptyTail (VS1 ++ VS2).
+Admitted.
+
+Fixpoint evalNonEmptyTail {e}{rho}{VS} (ev : eval rho e VS) : NonEmptyTail VS.
+  destruct ev; subst; eauto.
+  all: try eapply NonEmptyTail_singleton.
+  all: try solve [match goal with 
+    | [ H : TailSquash _ ?VS |- _ ] => move: H => [ _ h1 ] 
+    end; done].
+  - (* block *)
+    eapply NonEmptyTail_UNIONS; eauto.
+    intros V1 in1.
+    
+Admitted.
+
+(*
+Lemma evalNonEmptyTail : 
+  forall e rho VS, eval rho e VS -> NonEmptyTail VS.
+Proof.
+  induction 1.
+  all: subst.
+  all: auto.
+  all: try eapply NonEmptyTail_singleton.
+
+  (* true because we tail squashed *)
+  all: try solve [match goal with 
+    | [ H : TailSquash _ ?VS |- _ ] => move: H => [ _ h1 ] 
+    end; done].
+  - (* block *)
+
+  - (* choice *)
+    eapply NonEmptyTail_app; eauto.
+  - (* one *)
+    admit.
+  - (* all *)
+    admit.
+Admitted.
+*)
+
+End Theory.
+
+
+Module Rewrites.
+
+Ltac invert_eval := 
+  match goal with 
+  | [ H : eval ?rho (_ _) ?S |- _ ] => inversion H; subst; clear H 
+  | [ H : evalA ?rho (_ _) ?S |- _ ] => inversion H; subst; clear H 
+  | [ H : List.Forall2 (evalA _) (cons _ _) _ |- _ ] => 
+      inversion H; subst; clear H 
+  | [ H : List.Forall2 (evalA _) nil _ |- _ ] => 
+      inversion H; subst; clear H 
+  end.
+
+Lemma VarSwap : forall rho (x y : Ident) e, 
+    eval rho ((mini.Var x :=: mini.Var y) :>: e) ⊆
+    eval rho ((mini.Var y :=: mini.Var x) :>: e).
+Proof. 
+  intros.
+  intros VS vIn. unfold Ensembles.In in *.
+  invert_eval.
+  invert_eval.
+  invert_eval.
+  invert_eval.
+  cbn in H9.
+  eapply eval_Seq.
+Admitted.
+
+
+
+Lemma AppTup x rho v v0 v1: 
+  eval rho 
+  (mini.DefineV x :>: (mini.Var x :=: mini.Array [v0 ; v1])  :>: (mini.Var x :@: mini.Lit (common.Int v))) ⊆
+  eval rho (((mini.Lit (common.Int v) :=: mini.Lit (common.Int 0)) :>: v0) :|: ((mini.Lit (common.Int v) :=: mini.Lit (common.Int 1)) :>: v1)).
+Proof.
+  intros VS vIn. unfold Ensembles.In in *.
+  repeat invert_eval.
+  clear H4.
+  apply Squash_singleton_invert in H2. subst.
+Admitted.
+
+(*
+Lemma AppLam rho (x y :Ident) v e : 
+  eval rho 
+    (mini.DefineV y :>:
+       (mini.Var y :=: (mini.Fun Closed Succeeds x (mini.Var x) None e)) :>: 
+    (mini.ApplyD (mini.Var y) v)) ⊆
+  eval rho ((mini.DefineV x) :>: mini.Var x :=: v :>: e).
+Proof.
+  intros VS vIn. unfold Ensembles.In in *.
+  invert_eval.
+  invert_eval.
+  invert_eval.
+  invert_eval.
+  inversion H3. subst. clear H3.
+Admitted. *)
+
+End Rewrites.
