VerseRocq/verse/densem/squash.v
@@ -1,0 +1,190 @@
+Require Import Imports.
+
+From Stdlib Require Import Classes.EquivDec.
+Require Import structures.Sets.
+Require Import structures.List.
+
+Import SetNotations.
+Import SetMonadNotation.
+Import List.ListNotations.
+Import ListMonadNotation.
+
+Open Scope list_scope.
+Open Scope set_scope.
+
+
+(* This axiom is BAD. But convenient for now.... *)
+Axiom empty_dec : forall {A} (s : P A), 
+    { s ≃ ∅ } + { ~ (s ≃ ∅) }.
+
+Definition is_Empty_set {A} (s : P A) : bool := 
+  match empty_dec s with 
+  | left _ => true | right _ => false 
+  end.
+
+Lemma singleton_not_empty {A} {v : A} : ⌈ v ⌉ <> ∅. Admitted.
+
+Lemma notIn_singleton {A}{v : A} : ~ List.In ∅ [⌈ v ⌉]. 
+Proof.
+  intro h. inversion h.  apply singleton_not_empty in H. done. inversion H.
+Qed.
+
+
+(* ------------- functional squash -------------- *)
+
+(* squash using axiom *)
+Definition squash {A} (xs : list(P A)) : list (P A) := 
+  x <- xs ;; if is_Empty_set x then [x] else [].
+
+(* left to right squash, doesn't require axiom, but cannot 
+   produce a list.
+   fold_left allows us to use snoc in the definition of ALL
+*)
+Definition squash_fold_left {A B} (f : P A -> P B -> P A) : 
+  list (P B) -> P A -> P A := 
+  List.fold_left (fun bs x => If3 x (f bs x) bs).
+
+(* Find the first nonempty set, or an empty set if none exist. *)
+Definition first {A} (VS : list (P A)) : P A := 
+  squash_fold_left (fun xs x => x) VS ∅.
+
+(* squashing and picking at the same time *)
+
+Definition Cons {A} := (fun (V : P A) (VS : P (list A)) => 
+    v  ⭅ V  ;;  vs ⭅ VS ;; ⌈ v :: vs⌉).
+
+(* doesn't require axiom *)
+Fixpoint squash_pick {A} (xs : list (P A)) : P (list A) := 
+  match xs with 
+  | nil => ⌈ [] ⌉
+  | V :: VS => If3 V  
+               (Cons V (squash_pick VS))
+               (squash_pick VS)
+  end.
+
+(* -------------- Propositional Squash ------------ *)
+
+(* Squashed VS WS holds when WS := filter (fun x => x <> ∅) VS
+
+   NOTE: We cannot define this as a function (without using an axiom)
+   because results in Type cannot depend on Prop. But this relation 
+   is total and functional.
+*)
+Inductive Squash {A} : list (P A) -> list (P A) -> Prop := 
+  | sq_nil : Squash nil nil 
+  | sq_consIn : forall x xs ys,
+    x <> ∅ ->
+    Squash xs ys -> 
+    Squash (cons x xs) (cons x ys)
+  | sq_consOut : forall x xs ys,
+    x = ∅ ->
+    Squash xs ys -> 
+    Squash (cons x xs) ys.
+
+(* A success is any list that contains at least one nonempty VAL *)
+Definition Succeeds {A} (VS : P (list (P A))) : Prop :=
+  forall l, l ∈ VS -> exists v, v <> ∅ /\ List.In v l.
+
+Lemma Squash_functional {A} (VS : list (P A)) : forall WS1 WS2,
+      Squash VS WS1 -> Squash VS WS2 -> WS1 = WS2.
+Proof. 
+  induction VS; intros WS1 WS2 h1 h2; inversion h1; inversion h2; subst.
+  all: try done.
+  all: eauto.
+  - erewrite (IHVS ys ys0); auto.
+Qed.
+
+(* NOTE: Showing that Squash is functional requires classical reasoning. 
+   We need to know that 
+
+       forall any S, S = ∅ \/ S <> ∅
+
+   In order to prove this lemma:
+*)
+
+Lemma Squash_total {A} (decide_equality : forall (S:P A), S = ∅ \/ S <> ∅) 
+  : forall (VS : list (P A)), exists WS, Squash VS WS.
+Proof.
+  induction VS. exists nil. eapply sq_nil.
+  move: IHVS => [WS' IHWS'].
+  destruct (decide_equality a).
+  + exists WS'. eapply sq_consOut; auto.
+  + exists (a :: WS'). eapply sq_consIn; auto.
+Qed.
+
+(* The list is either empty, or the last element is inhabited. *)
+Definition NonEmptyTail {A} : list (P A) -> Prop := 
+  fun VS => 
+    match VS with 
+    | [] => True 
+    | _  => exists WS d, VS = WS ++ [d] /\ d <> ∅
+    end.
+
+Definition TailSquash {A} : list (P A) -> list (P A) -> Prop := 
+  fun VS WS => 
+    (exists n, VS = WS ++ List.repeat ∅ n) /\ NonEmptyTail WS.
+
+
+Lemma NonEmptyTail_nil {A} : @NonEmptyTail A [].
+done. Qed.
+Lemma NonEmptyTail_singleton {A}{v :A}: NonEmptyTail [ ⌈v⌉ ].
+cbn. exists nil. exists ⌈v⌉. cbv. split; auto; eapply singleton_not_empty. Qed.
+
+Lemma TailSquash_singleton {A} (v:A) VS : 
+  VS = [⌈ v ⌉] ->
+  TailSquash [⌈ v ⌉] VS.
+Proof. intros ->. unfold TailSquash. split. exists 0. cbn. auto.
+eapply NonEmptyTail_singleton; eauto. Qed.
+
+Lemma TailSquash_nil {A}  (VS : list (P A)) : 
+  VS = nil ->
+  TailSquash [] VS.
+Proof. intros ->. unfold TailSquash. split. exists 0. cbn. auto.
+eapply NonEmptyTail_nil; eauto. Qed.
+
+Lemma TailSquash_empty {A} (VS : list (P A)) : 
+  VS = nil ->
+  TailSquash [∅] VS.
+Proof. intros ->. unfold TailSquash. split. exists 1. cbn. auto.
+eapply NonEmptyTail_nil; eauto. Qed.
+
+Lemma noEmptyInSquash : forall {A} (xs ys : list (P A)), Squash xs ys -> 
+                                   not (List.In ∅ ys).
+Proof.
+  induction 1; unfold not; intros. inversion H.
+  inversion H1. contradiction. contradiction. contradiction.
+Qed.
+
+Lemma Squash_singleton {A} (v:A) VS : 
+  VS = [⌈ v ⌉] ->
+  Squash [⌈ v ⌉] VS.
+Proof. intros ->. eapply sq_consIn; eauto using singleton_not_empty.
+       eapply sq_nil. Qed.
+
+Lemma Squash_nil {A} (VS : list (P A)) : 
+  VS = nil ->
+  Squash [] VS.
+Proof. intros ->. eapply sq_nil. Qed.
+
+Hint Resolve 
+  singleton_not_empty 
+  NonEmptyTail_nil 
+  NonEmptyTail_singleton 
+  notIn_singleton
+  TailSquash_singleton
+  TailSquash_nil
+  TailSquash_empty
+  Squash_singleton
+  Squash_nil
+ : sets.
+
+Lemma Squash_singleton_invert {A} (v:A) VS : 
+  Squash [⌈ v ⌉] VS -> VS = [⌈ v ⌉].
+Proof. intro h. inversion h. subst. inversion H3. auto.
+subst. apply singleton_not_empty in H1. done. Qed.
+Lemma Squash_nil_invert {A} (VS : list (P A)) : 
+  Squash [] VS -> VS = [].
+Proof. intro h. inversion h. auto. Qed.
+Lemma Squash_empty_invert {A} (VS : list (P A)) : 
+  Squash [∅] VS -> VS = [].
+Proof. intro h. inversion h. done. inversion H3. done. Qed.
