VerseRocq/verse/structures/Imports.v
@@ -1,9 +1,16 @@
 Require Export ssreflect.
-Require Export Monad.
 From Stdlib Require Export Program.Equality.
 From Stdlib Require Export Classes.RelationClasses.
 From Stdlib Require Export Relations.Relation_Definitions.
 From Stdlib Require Export Classes.Morphisms.
+From Stdlib Require Import Classes.EquivDec.
+
+(* playing with fire. *)
+From Stdlib Require Export Sets.Classical_sets.
+From Stdlib Require Export Logic.PropExtensionality.
+From Stdlib Require Export Logic.FunctionalExtensionality.
+
+
 
 Ltac inv H := inversion H; try subst; clear H.
 
