VerseRocq/verse/structures/ListMonad.v
@@ -1,0 +1,51 @@
+Require Import Imports.
+From Stdlib Require Import Lists.List.
+
+Require Import structures.List.
+Require Import structures.Monad.
+Require Import structures.Laws.
+
+Import ListNotations.
+
+(* Monad definitions *)
+  
+
+#[export] Instance Functor_list : Functor list :=
+{ fmap := map }.
+
+#[export] Instance Monad_list : Monad list :=
+{ ret  := fun _ x => x :: nil; 
+  bind := fun _ _ x f =>  flat_map f x
+}.
+
+#[export] Instance Applicative_list : Applicative list :=
+{ pure := fun _ x => x :: nil;
+  ap   := @List.ap
+}.
+
+#[export] Instance Alternative_list : Alternative list :=
+  { empty := @nil ;
+    choose := @app
+  }.
+
+#[export] Instance Elem_list : Elem list := 
+  { elem := fun {A} ls x => @List.In A x ls }.
+
+
+(* Monad Laws *)
+
+#[export] Instance BindRetL_list : BindRetL (m:=list).
+intros A B f a. cbn. rewrite app_nil_r. done. Qed.
+
+#[export] Instance BindRetR_list : BindRetR (m:=list).
+intros A v. cbn. list_simpl. done. Qed.
+
+#[export] Instance BindBind_list : BindBind (m:=list).
+intros A B C ma f g. cbn. list_simpl. done. Qed.
+
+#[export] Instance RetInv_list : RetInv (m:=list).
+intros A a1 a2 h. cbn in h. inversion h. done.
+Qed.
+
+#[export] Instance BindRetInv_list : BindRetInv (m:=list).
+Abort.
