VerseRocq/verse/structures/NFSet.v
@@ -1,12 +1,10 @@
 Require Import Imports. 
-From Stdlib Require Import Logic.FunctionalExtensionality.
 
 Require Import structures.Sets.
 Require Import structures.List.
 
 Import SetNotations.
 Open Scope set_scope.
-Open Scope monad_scope.
 
 (* NONEMPTY FINITE SETS *)
 
